theories/crypto/CDH_RSR.ec
@@ -1,0 +1,2358 @@
+require import AllCore List Distr DBool DInterval DList SmtMap.
+require import FinType FSet NominalGroup PROM SplitRO2.
+
+import Distr.MRat.
+import DBool.Biased.
+import StdOrder.RealOrder.
+import RField.
+
+(* rangeset - move into Fset.ec *)
+
+lemma uniq_card_oflist (s : 'a list) : uniq s => card (oflist s) = size s.
+proof. by rewrite /card => /oflist_uniq/perm_eq_size => <-. qed.
+
+op rangeset (m n : int) = oflist (range m n).
+
+lemma card_rangeset m n : card (rangeset m n) = max 0 (n - m).
+proof. by rewrite uniq_card_oflist ?range_uniq size_range. qed.
+
+lemma mem_rangeset m n i : i \in rangeset m n <=> m <= i && i < n.
+proof. by rewrite mem_oflist mem_range. qed.
+
+(* Statistical distance - merge with SDist.ec *)
+
+op sdist : 'a distr -> 'a distr -> real.
+
+theory D.
+type in_t, out_t.
+op d1, d2 : out_t distr.
+
+clone FullRO as D1 with
+  type in_t    <- in_t,
+  type out_t   <- out_t,
+  op dout      <- fun _ => d1,
+  type d_in_t  <- unit,
+  type d_out_t <- bool.
+
+clone FullRO as D2 with
+  type in_t    <- in_t,
+  type out_t   <- out_t,
+  op dout      <- fun _ => d2,
+  type d_in_t  <- unit,
+  type d_out_t <- bool.
+
+module Wrap (O : D1.RO) : D1.RO = {
+  var dom : in_t fset
+
+  proc init() = {
+    dom <- fset0 ;
+    O.init();
+  }
+
+  proc get(x) = {
+    var r;
+
+    dom <- dom `|` fset1 x;
+    r <@ O.get(x);
+    return r;
+  }
+
+  proc set = O.set
+  proc rem = O.rem
+  proc sample = O.sample
+}.
+
+module type Distinguisher (O : D1.RO) = {
+  proc distinguish (_ : unit) : bool {O.get}
+}.
+
+axiom sdist_orcl (D <: Distinguisher) &m k :
+  (forall (O <: D1.RO{Wrap, D}),
+     hoare [D1.MainD(D, Wrap(O)).distinguish : true ==> card Wrap.dom <= k]) =>
+  `| Pr[D1.MainD(D, D1.RO).distinguish() @ &m : res] -
+     Pr[D1.MainD(D, D2.RO).distinguish() @ &m : res] | <=
+  k%r * sdist d1 d2.
+end D.
+
+clone import NominalGroup.NominalGroup as N.
+
+op e : Z.
+axiom e_EU : e \in EU.
+
+op elog (x : G) = choiceb (fun a => a \in EU /\ x = exp g a) e.
+
+op elogr (y : Z) (b : G) = choiceb (fun x => x \in EU /\ b = exp g (y * x)) e.
+
+lemma exprK (x y : Z) : x \in EU => y \in EU => elogr y (exp g (y * x)) = x.
+proof.
+move => x_EU y_EU; rewrite /elogr /=.
+have := choicebP (fun a : Z => a \in EU /\ exp g (y * x) = exp g (y * a)) e _;
+[by exists x | move => [E1 E2]].
+by apply (exp_inj' y) => //; rewrite -E2.
+qed.
+
+(* we only get one cancelation law *)
+lemma expK (x : Z) : x \in EU => elog (exp g x) = x.
+proof.
+move => x_EU; rewrite /elog /=.
+have [E1 E2] := choicebP (fun a : Z => a \in EU /\ exp g x = exp g a) e _;
+[by exists x | by apply exp_inj => //; rewrite -E2].
+qed.
+
+(* Does not seem to be used. *)
+lemma elog_EU x : elog x \in EU.
+proof.
+rewrite /elog; case (exists a, a \in EU /\ x = exp g a) => [E | nE].
+- by have /= := choicebP (fun a => a \in EU /\ x = exp g a) e E.
+by rewrite choiceb_dfl ?e_EU // /#.
+qed.
+
+(* Does not seem to be used. *)
+lemma dlist_EU n x xs :
+  xs \in dlist (duniform (elems EU)) n => x \in xs => x \in EU.
+proof.
+move => xs_d x_xs; rewrite memE -supp_duniform.
+move: xs_d; case (0 <= n) => Hn; 2: by rewrite supp_dlist0; smt().
+by rewrite supp_dlist // => -[? /allP H]; exact: H.
+qed.
+
+lemma fcard_oflist (s : 'a list) : card (oflist s) <= size s.
+proof.
+elim: s => [|x s IHs]; 1: by rewrite -set0E fcards0.
+by rewrite oflist_cons fcardU fcard1 /=; smt(fcard_ge0).
+qed.
+
+(* The CDH Game for Nominal Groups, with and without the factor for exponentiation *)
+theory NCDH.
+
+module type Adversary = {
+  proc solve (gx gy : G) : G
+}.
+
+module Game (A:Adversary) = {
+  proc main () : bool = {
+  var x, y, r;
+
+  x <$ duniform (elems EU);
+  y <$ duniform (elems EU);
+  r <@ A.solve(exp g x, exp g y);
+  return (r = exp g (x * y));
+  }
+}.
+
+module Game' (A:Adversary) = {
+  proc main () : bool = {
+  var x, y, r;
+
+  x <$ duniform (elems EU);
+  y <$ duniform (elems EU);
+  r <@ A.solve(g ^ x, g ^ y);
+  return (r = g ^ (x * y));
+  }
+}.
+
+module B (A : Adversary) = {
+  proc solve (gx gy : G) : G = {
+    var r;
+
+    r <@ A.solve(gx ^ inv f, gy ^ inv f);
+    return (r ^ f);
+  }
+}.
+
+(* If A wins against the "factor game", B(A) wins against the game w/o factors *)
+(* Should we relate to Game' for the final lemma? *)
+lemma unfactor (A <: Adversary) :
+  equiv[Game(A).main ~ Game'(B(A)).main : ={glob A} ==> res{1} => res{2}].
+proof.
+proc; inline *; auto.
+by call (: true) => //; auto; rewrite /exp => />; smt(mulA mulC powM pow_inv_f).
+qed.
+
+end NCDH.
+
+op na    : {int | 0 <= na}    as na_ge0.
+op nb    : {int | 0 <= nb}    as nb_ge0.
+op q_oa  : {int | 0 <= q_oa}  as q_oa_ge0.
+op q_ob  : {int | 0 <= q_ob}  as q_ob_ge0.
+op q_ddh : {int | 1 <= q_ddh} as q_ddh_ge1.
+
+module type CDH_RSR_Oracles = {
+  proc oA  (i : int) : G
+  proc oB  (j : int) : G
+  proc oa  (j : int) : Z
+  proc ob  (j : int) : Z
+  proc ddh (m : G, i j : int) : bool
+}.
+
+module type CDH_RSR_Oracles_i = {
+  include CDH_RSR_Oracles
+  proc init () : unit
+}.
+
+module type CDH_RSR_Oracles_i_xy = {
+  include CDH_RSR_Oracles
+  proc init (x y : Z) : unit
+}.
+
+module type Adversary (O : CDH_RSR_Oracles) = {
+  proc guess () : bool
+}.
+
+(* Counting wrapper for CDH_RSR Oracles *)
+module Count (O : CDH_RSR_Oracles) = {
+  var ca, cb, cddh : int
+
+  proc init () = {
+    ca   <- 0;
+    cb   <- 0;
+    cddh <- 0;
+  }
+
+  proc oa (i : int) = {
+    var r;
+
+    ca <- ca + 1;
+    r <@ O.oa(i);
+    return r;
+  }
+
+  proc ob (i : int) = {
+    var r;
+
+    cb <- cb + 1;
+    r <@ O.ob(i);
+    return r;
+  }
+
+  proc oA = O.oA
+  proc oB = O.oB
+
+  proc ddh (m, i, j) = {
+    var r;
+
+    cddh <- cddh + 1;
+    r <@ O.ddh(m, i, j);
+    return r;
+  }
+}.
+
+(* The actual CDH_RSR game: initialize oracles and counters and
+dispatach to adversary *)
+module Game (O : CDH_RSR_Oracles_i) (A : Adversary) = {
+  module O' = Count(O)
+
+  proc main () = {
+    var r;
+
+    O.init();
+    O'.init();
+    r <@ A(O').guess();
+    return r;
+  }
+}.
+
+module Game_xy (O : CDH_RSR_Oracles_i_xy) (A : Adversary) = {
+  module O' = Count(O)
+
+  proc main (x y : Z) = {
+    var r;
+
+    O.init(x, y);
+    O'.init();
+    r <@ A(O').guess();
+    return r;
+  }
+}.
+
+(* The games G1 and G2 are the "real" and the "ideal" game defined in
+cryptoprim.pdf *)
+clone import FullRO as FROZ with
+  type in_t    <- int,
+  type out_t   <- Z,
+  op dout      <- fun _ => dZ,
+  type d_in_t  <- unit,
+  type d_out_t <- bool.
+
+clone FROZ.MkRO as RAZ.
+clone FROZ.MkRO as RBZ.
+module OAZ = RAZ.RO.
+module OBZ = RBZ.RO.
+
+module G1 : CDH_RSR_Oracles  = {
+  proc init () = {
+    OAZ.init();
+    OBZ.init();
+  }
+
+  proc oa (i : int) = {
+    var a;
+
+    a <- e;
+    if (0 <= i < na) a <@ OAZ.get(i);
+    return a;
+  }
+
+  proc ob (j : int) = {
+    var b;
+
+    b <- e;
+    if (0 <= j < nb) b <@ OBZ.get(j);
+    return b;
+  }
+
+  proc oA (i : int) = {
+    var a;
+
+    a <- e;
+    if (0 <= i < na) a <@ OAZ.get(i);
+    return exp g a;
+  }
+
+  proc oB (j : int) = {
+    var b;
+
+    b <- e;
+    if (0 <= j < nb) b <@ OBZ.get(j);
+    return exp g b;
+  }
+
+  proc ddh (m, i, j) = {
+    var a, b, r;
+
+    a <- e;
+    b <- e;
+    r <- false;
+    if (0 <= i < na /\ 0 <= j < nb) {
+      a <@ OAZ.get(i);
+      b <@ OBZ.get(j);
+      r <- m = exp g (a * b);
+    }
+    return r;
+  }
+}.
+
+module G2 : CDH_RSR_Oracles = {
+  include G1 [oA, oB]
+  var ca, cb : int list
+
+  proc init () = {
+    G1.init();
+    ca <- [];
+    cb <- [];
+  }
+
+  proc oa (i : int) = {
+    var a;
+
+    a <- e;
+    if (0 <= i < na) {
+      ca <- i :: ca;
+      a <@ OAZ.get(i);
+    }
+    return a;
+  }
+
+  proc ob (j : int) = {
+    var b;
+
+    b <- e;
+    if (0 <= j < nb) {
+      cb <- j :: cb;
+      b <@ OBZ.get(j);
+    }
+    return b;
+  }
+
+  proc ddh (m, i, j) = {
+    var a, b, r;
+
+    a <- e;
+    b <- e;
+    r <- false;
+    if (0 <= i < na /\ 0 <= j < nb) {
+      a <@ OAZ.get(i);
+      b <@ OBZ.get(j);
+      if (i \in ca \/ j \in cb) {
+        r <- m = exp g (a * b);
+      }
+    }
+    return r;
+  }
+}.
+
+(* Intermediate games:
+- G sets "bad" where G1 and G2 differ
+- once "bad" has been set, G no longer logs queries to oa/ob *)
+module G (OA : FROZ.RO, OB : FROZ.RO) : CDH_RSR_Oracles = {
+  import var G2
+  var bad : bool
+
+  proc init () = {
+    OA.init();
+    OB.init();
+    ca  <- [];
+    cb  <- [];
+    bad <- false;
+  }
+
+  proc oa (i : int) = {
+    var a;
+
+    a <- e;
+    if (0 <= i < na) {
+      ca <- i :: ca;
+      a <@ OA.get(i);
+    }
+    return a;
+  }
+
+  proc ob (j : int) = {
+    var b;
+
+    b <- e;
+    if (0 <= j < nb) {
+      cb <- j :: cb;
+      b <@ OB.get(j);
+    }
+    return b;
+  }
+
+  proc oA (i : int) = {
+    var a;
+
+    a <- e;
+    if (0 <= i < na) a <@ OA.get(i);
+    return exp g a;
+  }
+
+  proc oB (j : int) = {
+    var b;
+
+    b <- e;
+    if (0 <= j < nb) b <@ OB.get(j);
+    return exp g b;
+  }
+
+  proc ddh (m, i, j) = {
+    var a, b, r, t;
+
+    a <- e;
+    b <- e;
+    r <- false;
+    t <- false;
+    if (0 <= i < na /\ 0 <= j < nb) {
+      a <@ OA.get(i);
+      b <@ OB.get(j);
+      t <- m = exp g (a * b);
+      if (i \in ca \/ j \in cb) {
+        r <- t;
+      } else {
+        bad <- bad \/ t;
+      }
+    }
+    return r;
+  }
+}.
+
+(* G' behaves like G, but samples invertible exponents (i.e. from EU *)
+clone import FullRO as FROEU with
+  type in_t   <- int,
+  type out_t  <- Z,
+  op dout     <- fun _ => duniform (elems EU),
+  type d_in_t <- unit,
+  type d_out_t <- bool.
+
+clone FROEU.MkRO as RAEU.
+clone FROEU.MkRO as RBEU.
+module OAEU = RAEU.RO.
+module OBEU = RBEU.RO.
+
+module G' = G(OAEU, OBEU).
+
+clone import Split as FROEU_S with
+  type in_t   <- int,
+  type out_t  <- Z,
+  op dout     <- fun _ => duniform (elems EU),
+  type d_in_t <- Z * Z,
+  type d_out_t <- bool.
+
+(* We could do with only 2 oracles for sampling A in EU for our proofs but,
+   with a view of having more meaningful names we do it with 3 oracles. *)
+
+clone FROEU.MkRO as REU.
+clone FROEU.MkRO as R0EU.
+clone FROEU.MkRO as R1EU.
+module OEU = REU.RO.
+module O0EU = R0EU.RO.
+module O1EU = R1EU.RO.
+
+(* Proof outline:
+
+1. |G1 - G2| = |G1b - G2b| <= G[bad]
+2. G[bad] <= G'[bad] + "prob. of distinguishing dZ and duniform EU"
+3. Define a game Gk that samples ia/ib and k \in [1..q_ddh] and show
+   Stop if oa(i) or ob(j) gets logged where ia[i]/ib[j] is true
+   G'[bad] <= q_ddh / ((1-pa)^q_oa * pa * (1 - pb)^q_ob * pb) Gk[ bad set at k-th call /\ !stop]
+4. Define simulation S and an adversary B against the NCDH games
+   Gk[ bad set at k-th call /\ !stop] <= S receives critical ddh call <= B wins NCDH game.
+*)
+
+(* Inner theory, parametric in the probability of inserting the NCDH problem *)
+abstract theory Inner.
+
+op pa, pb : real.
+axiom pa_bound : 0%r < pa && if q_oa = 0 then pa <= 1%r else pa < 1%r.
+axiom pb_bound : 0%r < pb && if q_ob = 0 then pb <= 1%r else pb < 1%r.
+
+(* the "simulation", called "A" in cryptoprim.pdf :
+
+We take gx and gy as parameters and use gx (rather than g) for
+oA(i) when ia[i] = true. In order for the simulation to remain in sync
+with the game G' (more precisely the intermediate game Gk' below), we
+need to align the randomness for a and b by multiplying/dividing by x
+(resp y) whenever ia[i] (resp ib[j]) is true. *)
+module S = {
+  import var G2
+  var cddh, k : int
+  var ia, ib  : bool list
+  var gx, gy  : G
+  var m_crit  : G
+
+  proc init (gx' : G, gy' : G) = {
+    ca   <- [];
+    cb   <- [];
+    cddh <- 0;
+    k    <$ [1..q_ddh];
+    ia   <$ dlist (dbiased pa) na;
+    ib   <$ dlist (dbiased pb) nb;
+    gx   <- gx';
+    gy   <- gy';
+    OAEU.init();
+    OBEU.init();
+  }
+
+  proc oa (i : int) = {
+    var a;
+
+    a <- e;
+    if (0 <= i < na) {
+      if (! nth false ia i){
+        ca <- i :: ca;
+        a <@ OAEU.get(i);
+      }
+    }
+    return a;
+  }
+
+  proc ob (j : int) = {
+    var b;
+
+    b <- e;
+    if (0 <= j < nb) {
+      if (! nth false ib j){
+        cb <- j :: cb;
+        b <@ OBEU.get(j);
+      }
+    }
+    return b;
+  }
+
+  proc oA (i : int) = {
+    var a, ga;
+
+    ga <- exp g e;
+    if (0 <= i < na) {
+      a <@ OAEU.get(i);
+      ga <- if nth false ia i then gx ^ a else exp g a;
+    }
+    return ga;
+  }
+
+  proc oB (j : int) = {
+    var b, gb;
+
+    gb <- exp g e;
+    if (0 <= j < nb) {
+      b <@ OBEU.get(j);
+      gb <- if nth false ib j then gy ^ b else exp g b;
+    }
+    return gb;
+  }
+
+  proc ddh (m, i, j) = {
+    var a, b, r;
+
+    a <- e;
+    b <- e;
+    r <- false;
+    cddh <- cddh + 1;
+    if (0 <= i < na /\ 0 <= j < nb) {
+      a <@ OAEU.get(i);
+      b <@ OBEU.get(j);
+      if (i \in ca \/ j \in cb) {
+        if (i \in ca) {
+          r <- m = (if nth false ib j then gy ^ b else exp g b) ^ a;
+        }
+        if (j \in cb) {
+          r <- m = (if nth false ia i then gx ^ a else exp g a) ^ b;
+        }
+      } else {
+          if (cddh = k) {
+            m_crit <- m ^ (inv a * inv b);
+        }
+      }
+    }
+    return r;
+  }
+}.
+
+module GameS (A : Adversary) = {
+  module O' = Count(S)
+
+  proc main(gx : G, gy : G) = {
+    var r;
+
+    S.init(gx, gy);
+    O'.init();
+    r <@ A(O').guess();
+    return r;
+  }
+}.
+
+(* adversary against CDH problem for nominal groups *)
+module B (A : Adversary) : NCDH.Adversary = {
+  proc solve(gx gy : G) : G = {
+    GameS(A).main(gx, gy);
+    return S.m_crit;
+  }
+}.
+
+clone import FullRO as FROG with
+  type in_t   <- int,
+  type out_t  <- G,
+  op dout     <- fun _ => dmap (duniform (elems EU)) (exp g),
+  type d_in_t <- unit,
+  type d_out_t <- bool.
+
+clone FROG.MkRO as R1G.
+module O1G = R1G.RO.
+
+op DELTA = (na + nb)%r * sdist dZ (duniform (elems EU)).
+
+lemma dEU_ll : is_lossless (duniform (elems EU)).
+proof. by smt(duniform_ll e_EU). qed.
+hint exact random : dEU_ll.
+
+lemma dG_ll : is_lossless (dmap (duniform (elems EU)) (exp g)).
+proof. by smt(dEU_ll dmap_ll). qed.
+
+section.
+
+declare module A : Adversary {G1, G2, G, S, Count,
+                              OAEU, OBEU, OEU, O0EU, O1EU, O1G}.
+
+axiom A_ll : forall (O <: CDH_RSR_Oracles{A}),
+  islossless O.oA =>
+  islossless O.oB =>
+  islossless O.oa =>
+  islossless O.ob =>
+  islossless O.ddh =>
+  islossless A(O).guess.
+
+axiom A_bound : forall (O <: CDH_RSR_Oracles{A}),
+  hoare [A(Count(O)).guess :
+         Count.ca = 0 /\ Count.cb = 0 /\ Count.cddh = 0 ==>
+         Count.ca <= q_oa /\ Count.cb <= q_ob /\ Count.cddh <= q_ddh].
+
+local module G1b = {
+  import var G2
+  include var G(OAZ, OBZ) [- ddh]
+
+  proc ddh (m, i, j) = {
+    var a, b, r;
+
+    a <- e;
+    b <- e;
+    r <- false;
+    if (0 <= i < na /\ 0 <= j < nb) {
+      a <@ OAZ.get(i);
+      b <@ OBZ.get(j);
+      r <- m = exp g (a * b);
+      bad <- bad \/ (r /\ ! (i \in ca \/ j \in cb));
+    }
+    return r;
+  }
+}.
+
+local lemma G1G2_Gbad &m :
+  `| Pr[Game(G1, A).main() @ &m : res] - Pr[Game(G2, A).main() @ &m : res] | <=
+  Pr[Game(G(OAZ, OBZ), A).main() @ &m : G.bad].
+proof.
+(* Introduce bad events into G1 and G2 *)
+have -> : Pr[Game(G1,  A).main() @ &m : res] =
+          Pr[Game(G1b, A).main() @ &m : res].
+- by byequiv => //; proc; inline *; sim.
+have -> : Pr[Game(G2,          A).main() @ &m : res] =
+          Pr[Game(G(OAZ, OBZ), A).main() @ &m : res].
+- byequiv => //; proc; inline *.
+  call (: ={OAZ.m, OBZ.m, G2.ca, G2.cb}); 1..4: (by sim); 2: by auto.
+  by proc; inline *; sp; if; auto.
+(* we can continue logging oa/ob queries once bad happens *)
+byequiv (_ : ={glob A} ==> ={G.bad} /\ (! G.bad{2} => ={res})) : G.bad => //;
+[proc; inline * | smt()].
+call (_ : G.bad, ={OAZ.m, OBZ.m, G2.ca, G2.cb, G.bad}, ={G.bad});
+  2..13: by (sim /> || (move => *; conseq />; islossless)).
+- by exact: A_ll.
+- proc; inline G1b.ddh G(OAZ, OBZ).ddh; sp.
+  if => //; 2: by auto.
+  wp; call (: ={OBZ.m}); 1: by sim.
+  call (: ={OAZ.m}); 1: by sim.
+  by auto => /> /#.
+- move => *; proc.
+  inline G1b.ddh; sp; if; auto.
+  by conseq (: true); [smt() | islossless].
+- move => *; proc.
+  inline G(OAZ, OBZ).ddh; sp; if; auto.
+  by conseq (: true); [smt() | islossless].
+- by auto => /> /#.
+qed.
+
+(** Expressing the games G, G' and G'' as distinguishers for statistical distance *)
+
+local clone import D as D_Z_EU with
+  type in_t   <- int,
+  type out_t  <- Z,
+  op d1       <- dZ,
+  op d2       <- duniform (elems EU).
+
+local module DisA (O : FROZ.RO) = {
+  module CG = Count(G(O, OBZ))
+
+  proc distinguish () = {
+    OBZ.init();
+    CG.init();
+    G2.ca <- [];
+    G2.cb <- [];
+    G.bad <- false;
+    A(CG).guess();
+    return G.bad;
+  }
+}.
+
+local module DisB (O : FROZ.RO) = {
+  module CG = Count(G(OAEU, O))
+
+  proc distinguish () = {
+    OAEU.init();
+    CG.init();
+    G2.ca <- [];
+    G2.cb <- [];
+    G.bad <- false;
+    A(CG).guess();
+    return G.bad;
+  }
+}.
+
+local lemma G_G' &m :
+  `| Pr[Game(G(OAZ, OBZ), A).main() @ &m : G.bad] -
+     Pr[Game(G',          A).main() @ &m : G.bad] | <= DELTA.
+proof.
+rewrite /DELTA.
+suff: `| Pr[Game(G(OAZ,  OBZ), A).main() @ &m : G.bad] -
+         Pr[Game(G(OAEU, OBZ), A).main() @ &m : G.bad] | <=
+      na%r * sdist dZ (duniform (elems EU)) /\
+      `| Pr[Game(G(OAEU, OBZ),  A).main() @ &m : G.bad] -
+         Pr[Game(G(OAEU, OBEU), A).main() @ &m : G.bad] | <=
+      nb%r * sdist dZ (duniform (elems EU)) by smt().
+split.
+- have -> : Pr[Game(G(OAZ,  OBZ), A).main() @ &m : G.bad] =
+            Pr[D1.MainD(DisA, D1.RO).distinguish() @ &m : res].
+  + byequiv => //; proc; inline *; auto.
+    call (: ={m}(OAZ, D1.RO) /\ ={OBZ.m, G2.ca, G2.cb, G.bad}); 1..5: by sim.
+    by auto.
+  have -> : Pr[Game(G(OAEU, OBZ), A).main() @ &m : G.bad] =
+            Pr[D1.MainD(DisA, D2.RO).distinguish() @ &m : res].
+  + byequiv => //; proc; inline *; auto.
+    call (: ={m}(OAEU, D2.RO) /\ ={OBZ.m, G2.ca, G2.cb, G.bad}); 1..5: by sim.
+    by auto.
+  apply (sdist_orcl DisA &m na) => O; proc; inline *; auto.
+  conseq (:_ ==> Wrap.dom \subset rangeset 0 na) => [_ _ I Isub|].
+  + apply (StdOrder.IntOrder.ler_trans (card (rangeset 0 na)));
+    [exact subset_leq_fcard | by rewrite card_rangeset /=; smt(na_ge0)].
+  call (: Wrap.dom \subset rangeset 0 na) => //.
+  + proc; inline *; sp; if; 2: (by auto); wp; call (: true); auto.
+    smt(in_fsetU in_fset1 mem_rangeset).
+  + proc; inline *; sp; if; by auto.
+  + proc; inline *; sp; if; 2: (by auto); wp; call (: true); auto.
+    smt(in_fsetU in_fset1 mem_rangeset).
+  + proc; inline *; sp; if; by auto.
+  + proc; inline *; sp; if; 2: (by auto); wp; rnd; wp.
+    call (: true); auto; smt(in_fsetU in_fset1 mem_rangeset).
+  + by inline *; wp; call (: true); auto; smt(in_fset0).
+- have -> : Pr[Game(G(OAEU, OBZ), A).main() @ &m : G.bad] =
+            Pr[D1.MainD(DisB, D1.RO).distinguish() @ &m : res].
+  + byequiv => //; proc; inline *; auto.
+    call (: ={m}(OBZ, D1.RO) /\ ={OAEU.m, G2.ca, G2.cb, G.bad}); 1..5: by sim.
+    by auto.
+  have -> : Pr[Game(G(OAEU, OBEU), A).main() @ &m : G.bad] =
+            Pr[D1.MainD(DisB, D2.RO).distinguish() @ &m : res].
+  + byequiv => //; proc; inline *; auto.
+    call (: ={m}(OBEU, D2.RO) /\ ={OAEU.m, G2.ca, G2.cb, G.bad}); 1..5: by sim.
+    by auto.
+  apply (sdist_orcl DisB &m nb) => O; proc; inline *; auto.
+  conseq (:_ ==> Wrap.dom \subset rangeset 0 nb) => [_ _ I Isub|].
+  + apply (StdOrder.IntOrder.ler_trans (card (rangeset 0 nb)));
+    [exact subset_leq_fcard | by rewrite card_rangeset /=; smt(nb_ge0)].
+  call (: Wrap.dom \subset rangeset 0 nb) => //.
+  + proc; inline *; sp; if; by auto.
+  + proc; inline *; sp; if; 2: (by auto); wp; call (: true); auto.
+    smt(in_fsetU in_fset1 mem_rangeset).
+  + proc; inline *; sp; if; by auto.
+  + proc; inline *; sp; if; 2: (by auto); wp; call (: true); auto.
+    smt(in_fsetU in_fset1 mem_rangeset).
+  + proc; inline *; sp; if; 2: (by auto); wp.
+    call (: true); auto; smt(in_fsetU in_fset1 mem_rangeset).
+  + by inline *; wp; call (: true); auto; smt(in_fset0).
+qed.
+
+local module Gk (OA : FROEU.RO, OB : FROEU.RO) : CDH_RSR_Oracles_i = {
+  import var G2 G
+  include var G(OA, OB) [oA, oB]
+  var cddh, i_k, j_k, k : int
+  var ia, ib            : bool list
+
+  proc init () = {
+    G(OA, OB).init();
+    cddh  <- 0;
+    i_k   <- -1;
+    j_k   <- -1;
+    k     <$ [1..q_ddh];
+    ia    <$ dlist (dbiased pa) na;
+    ib    <$ dlist (dbiased pb) nb;
+  }
+
+  proc oa (i : int) = {
+    var a;
+
+    a <- e;
+    if (0 <= i < na) {
+      if (i <> i_k) {
+        ca <- i :: ca;
+        a <@ OA.get(i);
+      }
+    }
+    return a;
+  }
+
+  proc ob (j : int) = {
+    var b;
+
+    b <- e;
+    if (0 <= j < nb) {
+      if (j <> j_k) {
+        cb <- j :: cb;
+        b <@ OB.get(j);
+      }
+    }
+    return b;
+  }
+
+  proc ddh (m, i, j) = {
+    var a, b, r, t;
+
+    a <- e;
+    b <- e;
+    r <- false;
+    t <- false;
+    cddh <- cddh + 1;
+    if (0 <= i < na /\ 0 <= j < nb) {
+      a <@ OA.get(i);
+      b <@ OB.get(j);
+      t <- m = exp g (a * b);
+      if (i \in ca \/ j \in cb) {
+        r <- t;
+      } else {
+          if (t /\ cddh = k /\ ! bad) {
+            bad <- true;
+            i_k <- i;
+            j_k <- j;
+        }
+      }
+    }
+    return r;
+  }
+}.
+
+(* Same as Gk, but record number of ddh query that sets bad. *)
+local module Gk_bad (OA : FROEU.RO, OB : FROEU.RO) : CDH_RSR_Oracles_i = {
+  import var G2 G
+  include var Gk(OA, OB) [oA, oB]
+  var k_bad   : int
+  var query_k : bool
+
+  proc init () = {
+    Gk(OA, OB).init();
+    k_bad   <- -1;
+    query_k <- false;
+  }
+
+  proc oa (i : int) = {
+    var a;
+
+    a <- e;
+    if (0 <= i < na) {
+      if (i <> i_k) {
+        ca <- i :: ca;
+        a <@ OA.get(i);
+      } else {
+        query_k <- true;
+      }
+    }
+    return a;
+  }
+
+  proc ob (j : int) = {
+    var b;
+
+    b <- e;
+    if (0 <= j < nb) {
+      if (j <> j_k) {
+        cb <- j :: cb;
+        b <@ OB.get(j);
+      } else {
+        query_k <- true;
+      }
+    }
+    return b;
+  }
+
+  proc ddh(m, i, j) = {
+    var a, b, r, t;
+
+    a <- e;
+    b <- e;
+    r <- false;
+    t <- false;
+    cddh <- cddh + 1;
+    if (0 <= i < na /\ 0 <= j < nb) {
+      a <@ OA.get(i);
+      b <@ OB.get(j);
+      t <- m = exp g (a * b);
+      if (i \in ca \/ j \in cb) {
+        r <- t;
+      } else {
+          if (t /\ ! bad) {
+            bad <- true;
+            k_bad <- cddh;
+            i_k <- i;
+            j_k <- j;
+        }
+      }
+    }
+    return r;
+  }
+}.
+
+op cs_all_false (bs : bool list) (is : int list) =
+  (forall i, i \in is => ! nth false bs i).
+
+op is_ok (bs : bool list) (is : int list) (i : int) =
+  cs_all_false bs is /\ nth false bs i.
+
+op nstop (ia ib : bool list) (ca cb : int list) =
+  cs_all_false ia ca /\ cs_all_false ib cb.
+
+(* should be an equality, but this suffices *)
+local lemma Gk_Gk_bad &m :
+  Pr[Game(Gk_bad(OAEU, OBEU), A).main() @ &m :
+     Gk.k = Gk_bad.k_bad /\
+     G.bad /\ is_ok Gk.ia G2.ca Gk.i_k /\ is_ok Gk.ib G2.cb Gk.j_k] <=
+  Pr[Game(Gk(OAEU, OBEU), A).main() @ &m :
+     G.bad /\ is_ok Gk.ia G2.ca Gk.i_k /\ is_ok Gk.ib G2.cb Gk.j_k].
+proof.
+byequiv => //; proc; inline *; symmetry.
+call (: G.bad /\ Gk.k <> Gk_bad.k_bad,
+
+        ={OAEU.m, OBEU.m, G2.ca, G2.cb, G.bad} /\
+        ={cddh, i_k, j_k, k}(Gk, Gk) /\
+        (G.bad <=> Gk.k = Gk_bad.k_bad){2});
+  try by (sim /> || (move => *; conseq />; islossless)).
+- by exact A_ll.
+- by proc; inline *; sp; if; auto => /#.
+- move => {&m} &m; proc; inline *; sp; if; auto; smt(dEU_ll).
+- by auto; smt(supp_dinter).
+qed.
+
+local lemma guess_bound &m :
+  1%r / q_ddh%r * (1%r - pa) ^ q_oa * (1%r - pb) ^ q_ob * pa * pb *
+  Pr[Game(G', A).main() @ &m : G.bad] <=
+  Pr[Game(Gk(OAEU, OBEU), A).main() @ &m :
+     G.bad /\ is_ok Gk.ia G2.ca Gk.i_k /\ is_ok Gk.ib G2.cb Gk.j_k].
+proof.
+pose p := Pr[Game(G', A).main() @ &m : G.bad].
+pose c := (1%r - pa) ^ q_oa * pa * (1%r - pb) ^ q_ob * pb.
+apply (ler_trans _ _ _ _ (Gk_Gk_bad &m)).
+byphoare (_ : glob A = (glob A){m} ==> _) => //.
+proc; inline *; swap [10..11] 6; swap 9 6.
+seq 14 : G.bad p (1%r / q_ddh%r * c) _ 0%r
+         (size G2.ca <= q_oa /\ size G2.cb <= q_ob /\
+          (G.bad => Gk_bad.k_bad \in [1..q_ddh] /\
+                    0 <= Gk.i_k < na /\ 0 <= Gk.j_k < nb) /\
+         ! (Gk.i_k \in G2.ca) /\ ! (Gk.j_k \in G2.cb));
+  4, 5: by auto; smt().
+- conseq (: _ ==> Count.cddh = Gk.cddh /\  0 <= Gk.cddh /\
+                  size G2.ca <= Count.ca /\ size G2.cb <= Count.cb /\
+                  (G.bad => (Gk.cddh <= q_ddh => Gk_bad.k_bad \in [1..q_ddh]) /\
+                            0 <= Gk.i_k < na /\ 0 <= Gk.j_k < nb) /\
+                  ! (Gk.i_k \in G2.ca) /\ ! (Gk.j_k \in G2.cb))
+         (: _ ==> Count.ca <= q_oa /\ Count.cb <= q_ob /\ Count.cddh <= q_ddh);
+  [ | smt () | seq 13 : (Count.ca = 0 /\ Count.cb = 0 /\ Count.cddh = 0) | ];
+  auto; 1: by call (A_bound (Gk_bad(OAEU, OBEU))).
+  call (: Count.cddh = Gk.cddh /\ 0 <= Gk.cddh /\
+          size G2.ca <= Count.ca /\ size G2.cb <= Count.cb /\
+          (G.bad => (Gk.cddh <= q_ddh => Gk_bad.k_bad \in [1..q_ddh]) /\
+                    0 <= Gk.i_k < na /\ 0 <= Gk.j_k < nb) /\
+          ! (Gk.i_k \in G2.ca) /\ ! (Gk.j_k \in G2.cb));
+    1, 2: (by proc; sp; if; [call (: true) | auto]); 4: by auto.
+  + proc; inline Gk_bad(OAEU, OBEU).oa; sp; wp.
+    by if; [if; [call (: true) | ] | ]; auto; smt().
+  + proc; inline Gk_bad(OAEU, OBEU).ob; sp; wp.
+    by if; [if; [call (: true) | ] | ]; auto; smt().
+  + proc; inline Gk_bad(OAEU, OBEU).ddh; sp; wp; if; 2: by auto; smt().
+    by auto; call (: true) => //; call (: true) => //; auto; smt(supp_dinter).
+- call (: (glob A) = (glob A){m} /\ OAEU.m = empty /\ OBEU.m = empty /\
+          G2.ca = [] /\ G2.cb = [] /\ G.bad = false /\
+          Gk.i_k = -1 /\ Gk.j_k = -1 /\
+          Gk_bad.query_k = false ==> G.bad); 2: by inline *; auto.
+  bypr=> &m' gA; rewrite /p.
+  byequiv (: ={glob A} /\ OAEU.m{2} = empty /\ OBEU.m{2} = empty /\
+             G2.ca{2} = [] /\ G2.cb{2} = [] /\ G.bad{2} = false /\
+             Gk.i_k{2} = -1 /\ Gk.j_k{2} = -1 /\
+             Gk_bad.query_k{2} = false ==> _); [ | smt() | done].
+  proc *; inline *; wp.
+  call (: Gk_bad.query_k,
+
+          ={OAEU.m, OBEU.m, G2.ca, G2.cb, G.bad} /\
+          ((0 <= Gk.i_k < na \/ 0 <= Gk.j_k < nb) => G.bad){2},
+
+          G.bad{2});
+    2..7, 9, 12: (by move => *; proc; inline *; sp; if; auto; smt(dEU_ll)).
+  + by exact A_ll.
+  + by proc; inline *; sp; if; [ | if{2} | ]; auto; smt().
+  + by move => *; proc; inline *; sp; if; [if | ]; auto; smt(dEU_ll).
+  + by proc; inline *; sp; if; [ | if{2} | ]; auto; smt().
+  + by move => *; proc; inline *; sp; if; [if | ]; auto; smt(dEU_ll).
+  + by proc; inline *; sp; if; auto; smt().
+  + by move => *; proc; inline *; sp; if; auto; smt(dEU_ll).
+  + by move => *; proc; inline *; sp; if; auto; smt(dEU_ll).
+  + by auto; smt().
+- seq 1 : (Gk.k = Gk_bad.k_bad) (1%r / q_ddh%r) c _ 0%r
+          (G.bad /\ size G2.ca <= q_oa /\ size G2.cb <= q_ob /\
+           0 <= Gk.i_k && Gk.i_k < na /\ 0 <= Gk.j_k && Gk.j_k < nb /\
+           ! (Gk.i_k \in G2.ca) /\ ! (Gk.j_k \in G2.cb));
+    1, 4, 5: by auto; smt().
+  + rnd; skip => &m' /> *; rewrite (mu_eq _ _ (pred1 Gk_bad.k_bad{m'})) //.
+    by rewrite dinter1E; smt (supp_dinter).
+  + rewrite /c => {c p}; pose p := (fun b => b = false).
+    pose IP := fun (cs : int list) (is : bool list) (n : int) =>
+                 forall (i : int), i \in oflist cs `&` oflist (range 0 n) =>
+                                     p (nth false is i).
+    pose JP := fun (c : int) (is : bool list) (n : int) =>
+                 forall (j : int), j \in fset1 c `&` oflist (range 0 n) =>
+                                   ! p (nth false is j).
+    have ? := pa_bound; have ? := pb_bound; have ? := na_ge0; have ? := nb_ge0.
+    seq 1 : (is_ok Gk.ia G2.ca Gk.i_k)
+            ((1%r - pa) ^ q_oa * pa) ((1%r - pb) ^ q_ob * pb) _ 0%r
+            (G.bad /\ Gk.k = Gk_bad.k_bad /\ size G2.cb <= q_ob /\
+             0 <= Gk.j_k && Gk.j_k < nb /\ ! (Gk.j_k \in G2.cb));
+      1, 4, 5: by auto; smt().
+    * rnd; skip => {&m} &m /> _ s_ca _ ik_ge0 ik_ltna _ _ ik_nca _.
+      rewrite (mu_eq_support _ _ (fun (x : bool list) =>
+                                    IP G2.ca{m} x na /\ JP Gk.i_k{m} x na));
+        1: by move => ia /= /(supp_dlist_size _ _ _ na_ge0) size_ia;
+              smt (fset1I in_filter mem_oflist mem_range nth_default nth_neg).
+      rewrite dlist_set2E //; 1: (by exact: dbiased_ll);
+        1..3: smt(mem_oflist mem_range in_fsetI in_fset1).
+      rewrite !dbiasedE /p /predC /= fset1I clamp_id 1: /#.
+      rewrite mem_oflist mem_range ik_ge0 ik_ltna /= fcard1 expr1.
+      apply ler_wpmul2r; 1: smt().
+      apply ler_wiexpn2l; smt(fcard_ge0 fcard_oflist subsetIl subset_leq_fcard).
+    * seq 1 : (is_ok Gk.ib G2.cb Gk.j_k)
+              ((1%r - pb) ^ q_ob * pb) 1%r _ 0%r
+              (G.bad /\ Gk.k = Gk_bad.k_bad /\ is_ok Gk.ia G2.ca Gk.i_k);
+        1, 3..5: by auto; smt().
+      rnd; skip => &m' /> _ s_cb jk_ge0 jk_ltnb jk_ncb _ _.
+      rewrite (mu_eq_support _ _ (fun (x : bool list) =>
+                                    IP G2.cb{m'} x nb /\ JP Gk.j_k{m'} x nb));
+        1: by move => ia /= /(supp_dlist_size _ _ _ nb_ge0) size_ia;
+              smt (fset1I in_filter mem_oflist mem_range nth_default nth_neg).
+      rewrite dlist_set2E //; 1: (by exact: dbiased_ll);
+        1..3: smt(mem_oflist mem_range in_fsetI in_fset1).
+      rewrite !dbiasedE /p /predC /= fset1I clamp_id 1: /#.
+      rewrite mem_oflist mem_range jk_ge0 jk_ltnb /= fcard1 expr1.
+      apply ler_wpmul2r; 1: smt().
+      apply ler_wiexpn2l; smt(fcard_ge0 fcard_oflist subsetIl subset_leq_fcard).
+qed.
+
+module type O = {
+  proc get_cs  ()        : int list
+  proc set_bad (i : int) : unit
+  proc oZ      (i : int) : Z
+  proc oG      (i : int) : G
+}.
+
+module type O_i = {
+  include O
+  proc init (n : int, is : bool list, x : Z) : unit
+}.
+
+module O_i_O (O : O_i) : O = {
+  proc get_cs  = O.get_cs
+  proc set_bad = O.set_bad
+  proc oZ      = O.oZ
+  proc oG      = O.oG
+}.
+
+module type DistinguisherO_i (O : O) = {
+  proc init   (x y : Z) : unit      {}
+  proc get_n  ()        : int       {}
+  proc get_is ()        : bool list {}
+  proc get_x  ()        : Z         {}
+  proc main   ()        : bool
+}.
+
+module D_i_D (D : DistinguisherO_i) (O : O) = {
+  proc main = D(O).main
+}.
+
+module MainDO (D : DistinguisherO_i) (O : O_i) = {
+  module D' = D(O)
+
+  proc init (x' y' : Z) = {
+    var is, n, x;
+
+    D'.init(x', y');
+    is <@ D'.get_is();
+    n  <@ D'.get_n();
+    x  <@ D'.get_x();
+    O.init(n, is, x);
+  }
+
+  proc main (x y : Z) = {
+    var r;
+
+    init(x, y);
+    r  <@ D(O_i_O(O)).main();
+    return r;
+  }
+}.
+
+local module Ok (O : FROEU.RO) : O_i = {
+  var n   : int
+  var cs  : int list
+  var bad : bool
+  var ik  : int
+  var is  : bool list
+  var x   : Z
+
+  proc init (n' : int, is' : bool list, x' : Z) = {
+    n   <- n';
+    is  <- is';
+    x   <- x';
+    cs  <- [];
+    bad <- false;
+    ik  <- -1;
+    O.init();
+  }
+
+  proc get_cs () = {
+    return cs;
+  }
+
+  proc set_bad (i : int) = {
+    if (0 <= i < n) {
+      if (! bad) {
+        bad <- true;
+        ik  <- i;
+      }
+    }
+  }
+
+  proc oZ (i : int) = {
+    var a;
+
+    a <- e;
+    if (0 <= i < n) {
+      if (i <> ik) {
+        cs <- i :: cs;
+        a <@ O.get(i);
+      }
+    }
+    return a;
+  }
+
+  proc oG (i : int) = {
+    var a;
+
+    a <- e;
+    if (0 <= i < n) a <@ O.get(i);
+    return exp g a;
+  }
+}.
+
+(* This is too lengthy and should be automated as
+   using RO_split is more tedious (due to having to define the various modules)
+   than redoing the same proof in the precise context.
+   Indeed Okt is about the same size as Ok2.
+   One would then need to add two lemmas to relate to a distinguisher.
+   Both of them would be about as short/long as Okt_Ok2.
+*)
+
+(*
+local module Okt (O : FROEUt.ROt) : O_i = {
+  import var G2 Gk Ok
+
+  proc init (n' : int, is' : bool list, x' : Z) = {
+    n   <- n';
+    is  <- is';
+    x   <- x';
+    cs  <- [];
+    bad <- false;
+    ik  <- -1;
+    O.init(nth false is);
+  }
+
+  proc get_cs () = {
+    return cs;
+  }
+
+  proc set_bad (i : int) = {
+    if (0 <= i < n) {
+      if (! bad) {
+        bad <- true;
+        ik  <- i;
+      }
+    }
+  }
+
+  proc oZ (i : int) = {
+    var a;
+
+    a <- e;
+    if (0 <= i < n) {
+      if (i <> ik) {
+        cs <- i :: cs;
+        a <@ O.get(i);
+      }
+    }
+    return a;
+  }
+
+  proc oG (i : int) = {
+    var a;
+
+    a <- e;
+    if (0 <= i < n) a <@ O.get(i);
+    return exp g a;
+  }
+}.
+*)
+
+local module Ok2 (O0 : FROEU.RO, O1 : FROEU.RO) : O_i = {
+  import var Ok
+
+  proc init (n' : int, is' : bool list, x' : Z) = {
+    n   <- n';
+    is  <- is';
+    x   <- x';
+    cs  <- [];
+    bad <- false;
+    ik  <- -1;
+    O0.init();
+    O1.init();
+  }
+
+  proc get_cs () = {
+    return cs;
+  }
+
+  proc set_bad (i : int) = {
+    if (0 <= i < n) {
+      if (! bad) {
+        bad <- true;
+        ik  <- i;
+      }
+    }
+  }
+
+  proc oZ (i : int) = {
+    var a;
+
+    a <- e;
+    if (0 <= i < n) {
+      if (i <> ik) {
+        cs <- i :: cs;
+        if (nth false is i) a <@ O1.get(i);
+        else                a <@ O0.get(i);
+      }
+    }
+    return a;
+  }
+
+  proc oG (i : int) = {
+    var a;
+
+    a <- e;
+    if (0 <= i < n) {
+      if (nth false is i) a <@ O1.get(i);
+      else                a <@ O0.get(i);
+    }
+    return exp g a;
+  }
+}.
+
+op splitO (m m0 m1 : (int, Z) fmap) (t : int -> bool) =
+  m = union_map m0 m1 /\
+  (forall x, x \in m1 =>   t x) /\
+  (forall x, x \in m0 => ! t x).
+
+local equiv Ok_Ok2 &m (D <: DistinguisherO_i {OEU, O0EU, O1EU, Ok}) :
+  MainDO(D, Ok(OEU)).main ~ MainDO(D, Ok2(O0EU, O1EU)).main :
+  ={arg, glob D} ==>
+  ={glob D} /\ ((is_ok Ok.is Ok.cs Ok.ik){1} <=> (is_ok Ok.is Ok.cs Ok.ik){2}).
+proof.
+proc *; inline *; wp.
+call (: ={glob Ok} /\ splitO OEU.m{1} O0EU.m{2} O1EU.m{2} (nth false Ok.is){2}).
+- by proc; auto.
+- by proc; auto.
+- proc; inline *; sp; if; [ | if; [ | sp; if{2} | ] | ]; auto.
+  + by smt(get_setE mergeE set_union_map_r).
+  + by smt(get_setE mergeE set_union_map_l).
+- proc; inline *; sp; if; 1, 3: by auto.
+  if{2}; auto; 1: smt(get_setE mem_set mergeE set_union_map_r).
+  by smt(get_setE mem_set mergeE set_union_map_l).
+- wp; call (: true); call (: true); call (: true); call (: true).
+  by auto; smt(mem_empty merge_empty).
+qed.
+
+local module Ok2X (O0 : FROEU.RO, O1 : FROG.RO) : O_i = {
+  import var Ok
+
+  proc init (n' : int, is' : bool list, x' : Z) = {
+    n   <- n';
+    is  <- is';
+    x   <- x';
+    cs  <- [];
+    bad <- false;
+    ik  <- -1;
+    O0.init();
+    O1.init();
+  }
+
+  proc get_cs () = {
+    return cs;
+  }
+
+  proc set_bad (i : int) = {
+    if (0 <= i < n) {
+      if (! bad) {
+        bad <- true;
+        ik  <- i;
+      }
+    }
+  }
+
+  proc oZ (i : int) = {
+    var a;
+
+    a <- e;
+    if (0 <= i < n) {
+      if (! nth false is i) {
+        cs <- i :: cs;
+        a <@ O0.get(i);
+      }
+    }
+    return a;
+  }
+
+  proc oG (i : int) = {
+    var a, ga;
+
+    a <- e;
+    ga <- exp g a;
+    if (0 <= i < n) {
+      if (nth false is i) { ga <@ O1.get(i); }
+      else                { a  <@ O0.get(i); ga <- exp g a; }
+    }
+    return ga;
+  }
+}.
+
+(* The up to bad reasoning that results in having a => and not a <=>
+   in the postcondition of the following equiv statement. *)
+local lemma Ok2_Ok2X &m (D <: DistinguisherO_i {O0EU, O1EU, O1G, Ok}) :
+  (forall (O <: O{D}),
+     islossless O.get_cs => islossless O.set_bad =>
+     islossless O.oZ => islossless O.oG =>
+     islossless D(O).main) =>
+  equiv[MainDO(D, Ok2(O0EU, O1EU)).main ~ MainDO(D, Ok2X(O0EU, O1G)).main :
+        ={arg, glob D} ==>
+        (is_ok Ok.is Ok.cs Ok.ik){1} => (is_ok Ok.is Ok.cs Ok.ik){2} /\
+                                        ={glob D}].
+proof.
+move => D_ll; proc *; inline *; wp; symmetry.
+call (: ! (cs_all_false Ok.is Ok.cs) \/
+        (Ok.bad /\ ! nth false Ok.is Ok.ik),
+
+        ={glob Ok, O0EU.m} /\ O1G.m{1} = map (fun _ => exp g) O1EU.m{2} /\
+        (forall r, r \in O1EU.m => oget (O1EU.m.[r]) \in EU){2} /\
+        (Ok.bad <=> 0 <= Ok.ik < Ok.n){2}).
+- by proc; auto.
+- by move => *; proc; auto.
+- by move => *; proc; auto.
+- by proc; auto.
+- by move => *; proc; auto.
+- by move => *; proc; auto => /#.
+- proc; inline *; sp; if; [auto | sp | auto].
+  if{2}; if{1}; try (sp; if{2}); auto; smt().
+- by move => *; proc; inline *; sp; if; [sp; if | ]; auto; smt(dEU_ll).
+- move => *; proc; inline *; sp.
+  by if; [sp; if; [sp; if | ] | ]; auto; smt(dEU_ll).
+- proc; inline *; sp; if; [ | if | ]; 1, 2, 4, 5: by auto.
+  seq 2 2 : (={x} /\ r{1} = exp g r{2} /\ r{2} \in EU /\
+             ((cs_all_false Ok.is Ok.cs) \/
+             (0 <= Ok.ik < Ok.n /\ ! nth false Ok.is Ok.ik)){2} /\
+             ={glob Ok, O0EU.m} /\ O1G.m{1} = map (fun _ => exp g) O1EU.m{2} /\
+             (forall r, r \in O1EU.m => oget (O1EU.m.[r]) \in EU){2} /\
+             (Ok.bad <=> 0 <= Ok.ik < Ok.n){2});
+    2: by if; auto; smt(get_setE get_set_sameE mapE map_set).
+  rnd elog (exp g); auto => /> *.
+  split => [|_]; 1: smt(expK supp_dmap supp_duniform).
+  split => [|_]; 2: smt(expK supp_dmap supp_duniform).
+  smt(dmap1E exp_inj mu_eq_support supp_duniform).
+- by move => *; proc; inline *; sp; if; [if | ]; auto; smt(dEU_ll dmap_ll).
+- by move => *; proc; inline *; sp; if; [if | ]; auto; smt(dEU_ll).
+- wp; call (: true); call (: true); call (: true); call (: true).
+  by auto; smt(mem_empty map_empty).
+qed.
+
+local module Ok2x (O0 : FROEU.RO, O1 : FROEU.RO) : O_i = {
+  import var Ok
+  include var Ok2(O0, O1) [- oZ, oG]
+
+  proc oZ (i : int) = {
+    var a;
+
+    a <- e;
+    if (0 <= i < n) {
+      if (! nth false is i) {
+        cs <- i :: cs;
+        a <@ O0.get(i);
+      }
+    }
+    return a;
+  }
+
+  proc oG (i : int) = {
+    var a;
+
+    a <- e;
+    if (0 <= i < n) {
+      if (nth false is i) { a <@ O1.get(i); a <- x * a; }
+      else                  a <@ O0.get(i);
+    }
+    return exp g a;
+  }
+}.
+
+lemma exp_exp_x x :
+  x \in EU =>
+  dmap (duniform (elems EU)) (exp g) =
+  dmap (duniform (elems EU)) (fun z => exp g (x * z)).
+proof.
+move => x_EU; rewrite !dmap_duniform; 1, 2: smt(exp_inj exp_inj').
+by apply eq_duniformP; move: (img_exp _ x_EU); smt(mem_oflist).
+qed.
+
+local lemma Ok2X_Ok2x &m x y (D <: DistinguisherO_i {O0EU, O1EU, O1G, Ok}) :
+  x \in EU =>
+  y \in EU =>
+  hoare [MainDO(D, Ok2x(O0EU, O1EU)).init :
+         fst arg \in EU /\ snd arg \in EU ==> Ok.x \in EU] =>
+  equiv[MainDO(D, Ok2X(O0EU, O1G)).main ~ MainDO(D, Ok2x(O0EU, O1EU)).main :
+        ={arg, glob D} /\ arg{1} = (x, y) ==>
+        ={glob D} /\
+        ((is_ok Ok.is Ok.cs Ok.ik){1} <=> (is_ok Ok.is Ok.cs Ok.ik){2})].
+proof.
+move => x_EU y_EU initP; proc *.
+inline MainDO(D, Ok2X(O0EU, O1G)).main MainDO(D, Ok2x(O0EU, O1EU)).main; wp.
+call (: ={glob Ok, O0EU.m} /\ Ok.x{1} \in EU /\
+        O1G.m{1} = (map (fun _ z => exp g (Ok.x * z)) O1EU.m){2}).
+- by proc; auto.
+- by proc; auto.
+- by proc; inline *; sp; if; [ | if | ]; auto => />.
+- proc; inline *; sp; if; [ | if; [ | sp | ] | ]; 1, 2, 4, 5: by auto.
+  seq 1 1 : (={x} /\ r{1} = exp g (Ok.x * r){2} /\
+             ={glob Ok, O0EU.m} /\ Ok.x{1} \in EU /\
+             O1G.m{1} = map (fun _ z => exp g (Ok.x{2} * z)) O1EU.m{2});
+    2: by if; auto; smt(get_setE get_set_sameE mapE map_set).
+  transitivity{1} { r <$ dmap (duniform (elems EU))
+                              (fun z => exp g (Ok.x * z)); }
+
+                  (={glob Ok, O0EU.m, O1G.m, x} /\ Ok.x{1} \in EU ==>
+                   ={glob Ok, O0EU.m, O1G.m, x, r} /\ Ok.x{1} \in EU)
+
+                  (={glob Ok, O0EU.m, x} /\ Ok.x{1} \in EU /\
+                   O1G.m{1} = map (fun _ z => exp g (Ok.x{2} * z)) O1EU.m{2} ==>
+                   r{1} = exp g (Ok.x{2} * r{2}) /\
+                   ={glob Ok, O0EU.m, x} /\ Ok.x{1} \in EU /\
+                   O1G.m{1} = map (fun _ z => exp g (Ok.x{2} * z)) O1EU.m{2});
+  [smt() | done | by auto => /> &2 *; rewrite (exp_exp_x Ok.x{2}); smt() | ].
+  rnd (elogr Ok.x{2}) (fun z => exp g (Ok.x{2} * z)); auto => /> *.
+  split => [|_]; 1: smt(exprK supp_dmap supp_duniform).
+  split => [*|_ r /supp_dmap [rx [/supp_duniform ? -> /=]]];
+    2: smt(exprK memE supp_duniform).
+  by rewrite dmap1E; smt(exp_inj' mu_eq_support supp_duniform).
+- conseq (: ={arg, glob D} ==>
+            ={glob D, glob Ok, O0EU.m} /\
+            O1G.m{1} = (map (fun _ z => exp g (Ok.x * z)) O1EU.m){2})
+         (: true ==> true) (: arg = (x, y) ==> Ok.x \in EU);
+  [by auto | by auto | by auto | by call initP; auto | inline *; wp].
+  call (: true); call (: true); call (: true); call (: true).
+  by auto; smt(map_empty).
+qed.
+
+local module Okx (O : FROEU.RO) : O_i = {
+  include var Ok(O) [- oZ, oG]
+
+  proc oZ (i : int) = {
+    var a;
+
+    a <- e;
+    if (0 <= i < n) {
+      if (! nth false is i) {
+        cs <- i :: cs;
+        a <@ O.get(i);
+      }
+    }
+    return a;
+  }
+
+  proc oG (i : int) = {
+    var a;
+
+    a  <- if (nth false is i) then inv x * e else e;
+    if (0 <= i < n) a <@ O.get(i);
+    return (exp g (if (nth false is i) then x * a else a));
+  }
+}.
+
+local lemma Ok2x_Okx &m x y (D <: DistinguisherO_i {OEU, O0EU, O1EU, Ok}) :
+  x \in EU =>
+  y \in EU =>
+  hoare [MainDO(D, Ok2x(O0EU, O1EU)).init :
+         fst arg \in EU /\ snd arg \in EU ==> Ok.x \in EU] =>
+  equiv[MainDO(D, Ok2x(O0EU, O1EU)).main ~ MainDO(D, Okx(OEU)).main :
+        ={arg, glob D} /\ arg{1} = (x, y) ==>
+        ={glob D} /\
+        ((is_ok Ok.is Ok.cs Ok.ik){1} <=> (is_ok Ok.is Ok.cs Ok.ik){2})].
+proof.
+move => x_EU y_EU initP; proc *.
+inline MainDO(D, Ok2x(O0EU, O1EU)).main MainDO(D, Okx(OEU)).main; wp.
+call (: Ok.x{1} \in EU /\ ={glob Ok} /\
+        splitO OEU.m{2} O0EU.m{1} O1EU.m{1} (nth false Ok.is){1}).
+- by proc; auto.
+- by proc; auto.
+- proc; inline *; sp; if; [ | if | ]; 1, 2, 4, 5: by auto.
+  by auto => />; smt(get_setE mergeE set_union_map_l).
+- proc; inline *; sp; if; 1, 3: by auto; smt(exp_inv mulA).
+  if{1}; auto; 1: smt(get_setE mem_set mergeE set_union_map_r).
+  by smt(get_setE mem_set mergeE set_union_map_l).
+- conseq (: ={arg, glob D} ==>
+            ={glob D, glob Ok} /\
+            splitO OEU.m{2} O0EU.m{1} O1EU.m{1} (nth false Ok.is){1})
+         (: arg = (x, y) ==> Ok.x \in EU) (: _ ==> _);
+  [by auto | by call initP; auto | by auto | inline *].
+  wp; call (: true); call (: true); call (: true); call (: true).
+  by auto; smt(mem_empty merge_empty).
+qed.
+
+local lemma Ok_Okx &m x y (D <: DistinguisherO_i {OEU, O0EU, O1EU, O1G, Ok}) :
+  x \in EU =>
+  y \in EU =>
+  (forall (O <: O{D}),
+     islossless O.get_cs => islossless O.set_bad =>
+     islossless O.oZ => islossless O.oG =>
+     islossless D(O).main) =>
+  hoare [MainDO(D, Ok2x(O0EU, O1EU)).init :
+         fst arg \in EU /\ snd arg \in EU ==> Ok.x \in EU] =>
+  equiv [MainDO(D, Ok(OEU)).main ~ MainDO(D, Okx(OEU)).main :
+        ={arg, glob D} /\ arg{1} = (x, y) ==>
+        (is_ok Ok.is Ok.cs Ok.ik){1} => (is_ok Ok.is Ok.cs Ok.ik){2} /\
+                                        ={glob D}].
+proof.
+move => x_EU y_EU D_ll initP.
+transitivity MainDO(D, Ok2(O0EU, O1EU)).main
+
+             (={arg, glob D} ==>
+              ={glob D} /\
+              ((is_ok Ok.is Ok.cs Ok.ik){1} <=> (is_ok Ok.is Ok.cs Ok.ik){2}))
+
+             (={arg, glob D} /\ arg{1} = (x, y) ==>
+              (is_ok Ok.is Ok.cs Ok.ik){1} => (is_ok Ok.is Ok.cs Ok.ik){2} /\
+                                              ={glob D});
+  1, 2: smt(); 1: by exact (Ok_Ok2 &m D).
+transitivity MainDO(D, Ok2X(O0EU, O1G)).main
+
+             (={arg, glob D} ==>
+              (is_ok Ok.is Ok.cs Ok.ik){1} => (is_ok Ok.is Ok.cs Ok.ik){2} /\
+                                              ={glob D})
+
+             (={arg, glob D} /\ arg{1} = (x, y) ==>
+              ={glob D} /\
+              ((is_ok Ok.is Ok.cs Ok.ik){1} <=> (is_ok Ok.is Ok.cs Ok.ik){2}));
+  1, 2: smt(); 1: by exact (Ok2_Ok2X &m D D_ll).
+transitivity MainDO(D, Ok2x(O0EU, O1EU)).main
+
+             (={arg, glob D} /\ arg{1} = (x, y) ==>
+              ={glob D} /\
+              ((is_ok Ok.is Ok.cs Ok.ik){1} <=> (is_ok Ok.is Ok.cs Ok.ik){2}))
+
+             (={arg, glob D} /\ arg{1} = (x, y) ==>
+              ={glob D} /\
+              ((is_ok Ok.is Ok.cs Ok.ik){1} <=> (is_ok Ok.is Ok.cs Ok.ik){2}));
+  1, 2: smt(); 1: by exact (Ok2X_Ok2x &m x y D x_EU y_EU initP).
+by exact (Ok2x_Okx &m x y D x_EU y_EU initP).
+qed.
+
+local module GkD (OA : O, OB : FROEU.RO) = {
+  import var G2 G Gk
+  var x, y : Z
+
+  proc init_var (x' y' : Z) = {
+    ca    <- [];
+    cb    <- [];
+    bad   <- false;
+    cddh  <- 0;
+    i_k   <- -1;
+    j_k   <- -1;
+    k     <$ [1..q_ddh];
+    ia    <$ dlist (dbiased pa) na;
+    ib    <$ dlist (dbiased pb) nb;
+    x     <- x';
+    y     <- y';
+  }
+
+  proc get_n () = {
+    return na;
+  }
+
+  proc get_is () = {
+    return ia;
+  }
+
+  proc get_x () = {
+    return x;
+  }
+
+  proc oa = OA.oZ
+
+  proc ob (j : int) = {
+    var b;
+
+    b <- e;
+    if (0 <= j < nb) {
+      if (j <> j_k) {
+        cb <- j :: cb;
+        b <@ OB.get(j);
+      }
+    }
+    return b;
+  }
+
+  proc oA = OA.oG
+
+  proc oB (j : int) = {
+    var b;
+
+    b <- e;
+    if (0 <= j < nb) b <@ OB.get(j);
+    return exp g b;
+  }
+
+  proc ddh (m, i, j) = {
+    var a, b, ca, r, t;
+
+    a <- g;
+    b <- e;
+    r <- false;
+    t <- false;
+    cddh <- cddh + 1;
+    if (0 <= i < na /\ 0 <= j < nb) {
+      a  <@ OA.oG(i);
+      b  <@ OB.get(j);
+      ca <@ OA.get_cs();
+      t <- m = a ^ b;
+      if (i \in ca \/ j \in cb) {
+        r <- t;
+      } else {
+          if (t /\ cddh = k /\ ! bad) {
+            bad <- true;
+            i_k <- i;
+            j_k <- j;
+            OA.set_bad(i);
+        }
+      }
+    }
+    return r;
+  }
+}.
+
+local module Dk (OA : O) = {
+  module O  = GkD(OA, OBEU)
+  module CO = Count(O)
+
+  proc init (x y : Z) = {
+    O.init_var(x, y);
+    OBEU.init();
+  }
+
+  proc get_n = O.get_n
+  proc get_is = O.get_is
+  proc get_x = O.get_x
+
+  proc main () = {
+    var r;
+
+    CO.init();
+    r <@ A(Count(CO)).guess();
+    return r;
+  }
+}.
+
+local lemma Dk_ll (O <: O{Dk}) :
+  islossless O.get_cs =>
+  islossless O.set_bad =>
+  islossless O.oZ =>
+  islossless O.oG =>
+  islossless Dk(O).main.
+proof.
+move => get_cs_ll set_bad_ll oZ_ll oG_ll; proc; inline *; call (: true); auto.
+- by exact A_ll.
+- by proc; inline *; sp; if; auto; smt(dEU_ll).
+- by proc; inline *; wp; call (oZ_ll); auto.
+- by proc; inline *; sp; if; [if | ]; auto; smt(dEU_ll).
+- proc; inline *; sp; if; 2: by auto; smt(dEU_ll).
+  seq 7 : true; auto; 2: by if; [ | if]; auto; call set_bad_ll; auto.
+  by swap 1 2; call (get_cs_ll); wp; call (oG_ll); auto; smt(dEU_ll).
+qed.
+
+local lemma Dk_initP :
+  hoare [MainDO(Dk, Ok2x(O0EU, O1EU)).init :
+         fst arg \in EU /\ snd arg \in EU ==> Ok.x \in EU].
+proof. by proc; inline *; auto. qed.
+
+local module Gkx (OA : FROEU.RO, OB : FROEU.RO) : CDH_RSR_Oracles_i_xy = {
+  import var G2 G Gk
+  include var Gk(OA, OB) [ob, oB]
+  var x, y : Z
+
+  proc init (x' y' : Z) = {
+    Gk(OA, OB).init();
+    x <- x';
+    y <- y';
+  }
+
+  proc oa (i : int) = {
+    var a;
+
+    a <- e;
+    if (0 <= i < na) {
+      if (! nth false ia i) {
+        ca <- i :: ca;
+        a <@ OA.get(i);
+      }
+    }
+    return a;
+  }
+
+  proc oA(i : int) = {
+    var a;
+
+    a  <- if (nth false ia i) then inv x * e else e;
+    if (0 <= i < na) a <@ OA.get(i);
+    return (exp g (if (nth false ia i) then x * a else a));
+  }
+
+  proc ddh (m, i, j) = {
+    var a, b, r, t;
+
+    a <- e;
+    b <- e;
+    r <- false;
+    t <- false;
+    cddh <- cddh + 1;
+    if (0 <= i < na /\ 0 <= j < nb) {
+      a <@ OA.get(i);
+      b <@ OB.get(j);
+      t <- m = exp g ((if (nth false ia i) then x * a else a) * b);
+      if (i \in ca \/ j \in cb) {
+        r <- t;
+      } else {
+          if (t /\ cddh = k /\ ! bad) {
+            bad <- true;
+            i_k <- i;
+            j_k <- j;
+        }
+      }
+    }
+    return r;
+  }
+}.
+
+local lemma Gk_Gkx &m x y :
+  x \in EU =>
+  y \in EU =>
+  Pr[Game   (Gk (OAEU, OBEU), A).main(    ) @ &m :
+     G.bad /\ is_ok Gk.ia G2.ca Gk.i_k /\ is_ok Gk.ib G2.cb Gk.j_k] <=
+  Pr[Game_xy(Gkx(OAEU, OBEU), A).main(x, y) @ &m :
+     G.bad /\ is_ok Gk.ia G2.ca Gk.i_k /\ is_ok Gk.ib G2.cb Gk.j_k].
+proof.
+move => x_EU y_EU.
+have -> :   Pr[Game(Gk(OAEU, OBEU), A).main() @ &m :
+               G.bad /\ is_ok Gk.ia G2.ca Gk.i_k /\ is_ok Gk.ib G2.cb Gk.j_k] =
+            Pr[MainDO(Dk, Ok(OEU)).main(x, y) @ &m :
+               G.bad /\ is_ok Ok.is Ok.cs Ok.ik /\ is_ok Gk.ib G2.cb Gk.j_k].
+- byequiv => //; proc; inline *; wp.
+  call (: ={OBEU.m, G2.cb, G.bad} /\ ={m}(OAEU, OEU) /\
+          ={cddh, j_k, k, ia, ib}(Gk, Gk) /\
+          G2.ca{1} = Ok.cs{2} /\ Gk.i_k{1} = Ok.ik{2} /\ Gk.ia{1} = Ok.is{2} /\
+          (G.bad = Ok.bad /\ Ok.n = na){2});
+    1, 2, 4: (by proc; inline *; sp; if; try if; auto); 3: by auto.
+  + by proc; inline *; sp; if; [ | if | ]; auto; smt().
+  + proc; inline Gk(OAEU, OBEU).ddh Count(GkD(O_i_O(Ok(OEU)), OBEU)).ddh.
+    inline GkD(O_i_O(Ok(OEU)), OBEU).ddh O_i_O(Ok(OEU)).get_cs.
+    sp; if; 1, 3: by auto.
+    seq 3 4 : (={OBEU.m, G2.cb, G.bad, t} /\ ={m}(OAEU, OEU) /\
+               ={cddh, j_k, k, ia, ib}(Gk, Gk) /\
+               G2.ca{1} = Ok.cs{2} /\ Gk.i_k{1} = Ok.ik{2} /\
+               Gk.ia{1} = Ok.is{2} /\
+               (G.bad = Ok.bad /\ Ok.n = na){2} /\
+               i0{1} = i1{2} /\ j0{1} = j1{2} /\ r0{1} = r1{2} /\
+               G2.ca{1} = ca{2} /\ 0 <= i0{1} < na);
+      2: by inline *; auto => />.
+    wp; call (: ={OBEU.m}); auto.
+    by inline *; sp; rcondt{2} 1; auto; smt(expM).
+apply (ler_trans (Pr[MainDO(Dk, Okx(OEU)).main(x, y) @ &m :
+                     G.bad /\ is_ok Ok.is Ok.cs Ok.ik /\
+                              is_ok Gk.ib G2.cb Gk.j_k])).
+byequiv (: ={arg, glob Dk} /\ arg{1} = (x, y) ==> _) => //.
+conseq (Ok_Okx &m x y Dk x_EU y_EU Dk_ll Dk_initP); smt().
+byequiv (: ={glob A, x, y} /\ fst arg{1} = x /\ snd arg{1} = y ==> _) => //.
+proc; inline *; wp.
+call (: ={OBEU.m, G2.cb, G.bad} /\ ={m}(OEU, OAEU) /\
+        ={cddh, j_k, k, ia, ib}(Gk, Gk) /\
+        Ok.cs{1} = G2.ca{2} /\ Ok.ik{1} = Gk.i_k{2} /\
+        Ok.is{1} = Gk.ia{2} /\ Ok.x{1} = Gkx.x{2} /\
+        (G.bad = Ok.bad /\ Ok.n = na){1});
+  1..4: (by proc; inline *; sp; if; try if; auto); 2: by auto.
+- proc; inline Gkx(OAEU, OBEU).ddh Count(GkD(O_i_O(Okx(OEU)), OBEU)).ddh.
+  inline GkD(O_i_O(Okx(OEU)), OBEU).ddh O_i_O(Ok(OEU)).get_cs.
+  sp; if; 1, 3: by auto.
+  seq 4 3 : (={OBEU.m, G2.cb, G.bad, t} /\ ={m}(OEU, OAEU) /\
+             ={cddh, j_k, k, ia, ib}(Gk, Gk) /\
+             Ok.cs{1} = G2.ca{2} /\ Ok.ik{1} = Gk.i_k{2} /\
+             Ok.is{1} = Gk.ia{2} /\ Ok.x{1} = Gkx.x{2} /\
+             (G.bad = Ok.bad /\ Ok.n = na){1} /\
+             i1{1} = i0{2} /\ j1{1} = j0{2} /\ r1{1} = r0{2} /\
+             ca{1} = G2.ca{2} /\ 0 <= i1{1} < na); 2: by inline *; auto => />.
+  wp; call (: ={OBEU.m}); auto.
+  by inline *; sp; rcondt{1} 1; auto; smt(expM).
+qed.
+
+local module GkxD (OA : FROEU.RO, OB : O) = {
+  import var G2 G Gk
+  var x, y : Z
+
+  proc init_var (x' y' : Z) = {
+    ca    <- [];
+    cb    <- [];
+    bad   <- false;
+    cddh  <- 0;
+    i_k   <- -1;
+    j_k   <- -1;
+    k     <$ [1..q_ddh];
+    ia    <$ dlist (dbiased pa) na;
+    ib    <$ dlist (dbiased pb) nb;
+    x     <- x';
+    y     <- y';
+  }
+
+  proc get_n () = {
+    return nb;
+  }
+
+  proc get_is () = {
+    return ib;
+  }
+
+  proc get_x () = {
+    return y;
+  }
+
+  proc oa (i : int) = {
+    var a;
+
+    a <- e;
+    if (0 <= i < na) {
+      if (! nth false ia i) {
+        ca <- i :: ca;
+        a <@ OA.get(i);
+      }
+    }
+    return a;
+  }
+
+  proc ob = OB.oZ
+
+  proc oA(i : int) = {
+    var a;
+
+    a  <- if (nth false ia i) then inv x * e else e;
+    if (0 <= i < na) a <@ OA.get(i);
+    return (exp g (if (nth false ia i) then x * a else a));
+  }
+
+  proc oB = OB.oG
+
+  proc ddh (m, i, j) = {
+    var a, b, cb, r, t;
+
+    a <- e;
+    b <- g;
+    r <- false;
+    t <- false;
+    cddh <- cddh + 1;
+    if (0 <= i < na /\ 0 <= j < nb) {
+      a  <@ OA.get(i);
+      b  <@ OB.oG(j);
+      cb <@ OB.get_cs();
+      t <- m = b ^ (if (nth false ia i) then x * a else a);
+      if (i \in ca \/ j \in cb) {
+        r <- t;
+      } else {
+          if (t /\ cddh = k /\ ! bad) {
+            bad <- true;
+            i_k <- i;
+            j_k <- j;
+            OB.set_bad(j);
+        }
+      }
+    }
+    return r;
+  }
+}.
+
+local module Dkx (OB : O) = {
+  module O  = GkxD(OAEU, OB)
+  module CO = Count(O)
+
+  proc init (x y : Z) = {
+    O.init_var(x, y);
+    OAEU.init();
+  }
+
+  proc get_n = O.get_n
+  proc get_is = O.get_is
+  proc get_x = O.get_x
+
+  proc main () = {
+    var r;
+
+    CO.init();
+    r <@ A(Count(CO)).guess();
+    return r;
+  }
+}.
+
+local lemma Dkx_ll (O <: O{Dkx}) :
+  islossless O.get_cs =>
+  islossless O.set_bad =>
+  islossless O.oZ =>
+  islossless O.oG =>
+  islossless Dkx(O).main.
+proof.
+move => get_cs_ll set_bad_ll oZ_ll oG_ll; proc; inline *; call (: true); auto.
+- by exact A_ll.
+- by proc; inline *; sp; if; auto; smt(dEU_ll).
+- by proc; inline *; sp; if; [if | ]; auto; smt(dEU_ll).
+- by proc; inline *; wp; call (oZ_ll); auto.
+- proc; inline *; sp; if; 2: by auto; smt(dEU_ll).
+  seq 7 : true; auto; 2: by if; [ | if]; auto; call set_bad_ll; auto.
+  by call (get_cs_ll); wp; call (oG_ll); auto; smt(dEU_ll).
+qed.
+
+local lemma Dkx_initP :
+  hoare [MainDO(Dkx, Ok2x(O0EU, O1EU)).init :
+         fst arg \in EU /\ snd arg \in EU ==> Ok.x \in EU].
+proof. by proc; inline *; auto. qed.
+
+local module Gkxy (OA : FROEU.RO, OB : FROEU.RO) : CDH_RSR_Oracles_i_xy = {
+  import var G2 G Gk GkD
+  include var Gkx(OA, OB) [- ob, oB, ddh]
+
+  proc ob (j : int) = {
+    var b;
+
+    b <- e;
+    if (0 <= j < nb) {
+      if (! nth false ib j) {
+        cb <- j :: cb;
+        b <@ OB.get(j);
+      }
+    }
+    return b;
+  }
+
+  proc oB(j : int) = {
+    var b;
+
+    b  <- if (nth false ib j) then inv y * e else e;
+    if (0 <= j < nb) {
+      b <@ OB.get(j);
+    }
+    return (exp g (if (nth false ib j) then y * b else b));
+  }
+
+  proc ddh (m, i, j) = {
+    var a, b, r, t;
+
+    a <- e;
+    b <- e;
+    r <- false;
+    t <- false;
+    cddh <- cddh + 1;
+    if (0 <= i < na /\ 0 <= j < nb) {
+      a <@ OA.get(i);
+      b <@ OB.get(j);
+      t <- m = exp g ((if (nth false ia i) then x * a else a) *
+                      (if (nth false ib j) then y * b else b));
+      if (i \in ca \/ j \in cb) {
+        r <- t;
+      } else {
+          if (t /\ cddh = k /\ ! bad) {
+            bad <- true;
+            i_k <- i;
+            j_k <- j;
+        }
+      }
+    }
+    return r;
+  }
+}.
+
+local lemma Gkx_Gkxy &m x y :
+  x \in EU =>
+  y \in EU =>
+  Pr[Game_xy(Gkx (OAEU, OBEU), A).main(x, y) @ &m :
+     G.bad /\ is_ok Gk.ia G2.ca Gk.i_k /\ is_ok Gk.ib G2.cb Gk.j_k] <=
+  Pr[Game_xy(Gkxy(OAEU, OBEU), A).main(x, y) @ &m :
+     G.bad /\ is_ok Gk.ia G2.ca Gk.i_k /\ is_ok Gk.ib G2.cb Gk.j_k].
+proof.
+move => x_EU y_EU.
+have -> :   Pr[Game_xy(Gkx(OAEU, OBEU), A).main(x, y) @ &m :
+               G.bad /\ is_ok Gk.ia G2.ca Gk.i_k /\ is_ok Gk.ib G2.cb Gk.j_k] =
+            Pr[MainDO(Dkx, Ok(OEU)).main(x, y) @ &m :
+               G.bad /\ is_ok Gk.ia G2.ca Gk.i_k /\ is_ok Ok.is Ok.cs Ok.ik].
+- byequiv => //; proc; inline *; wp.
+  call (: ={OAEU.m, G2.ca, G.bad} /\ ={m}(OBEU, OEU) /\
+          ={cddh, i_k, k, ia, ib}(Gk, Gk) /\ ={x}(Gkx, GkxD) /\
+          G2.cb{1} = Ok.cs{2} /\ Gk.j_k{1} = Ok.ik{2} /\ Gk.ib{1} = Ok.is{2} /\
+          (G.bad = Ok.bad /\ Ok.n = nb){2});
+    2..4: (by proc; inline *; sp; if; try if; auto); 3: by auto.
+  + by proc; inline *; sp; if; auto; smt().
+  + proc; inline Gkx(OAEU, OBEU).ddh Count(GkxD(OAEU, O_i_O(Ok(OEU)))).ddh.
+    inline GkxD(OAEU, O_i_O(Ok(OEU))).ddh O_i_O(Ok(OEU)).get_cs.
+    sp; if; 1, 3: by auto.
+    seq 3 4 : (={OAEU.m, G2.ca, G.bad, t} /\ ={m}(OBEU, OEU) /\
+               ={cddh, i_k, k, ia, ib}(Gk, Gk) /\ ={x}(Gkx, GkxD) /\
+               G2.cb{1} = Ok.cs{2} /\ Gk.j_k{1} = Ok.ik{2} /\
+               Gk.ib{1} = Ok.is{2} /\
+               (G.bad = Ok.bad /\ Ok.n = nb){2} /\
+               i0{1} = i1{2} /\ j0{1} = j1{2} /\ r0{1} = r1{2} /\
+               G2.cb{1} = cb{2} /\ 0 <= j0{1} < nb);
+      2: by inline *; auto => />.
+    swap 1 1; wp; call (: ={OAEU.m}); auto.
+    by inline *; sp; rcondt{2} 1; auto; smt(expM mulC).
+apply (ler_trans (Pr[MainDO(Dkx, Okx(OEU)).main(x, y) @ &m :
+                     G.bad /\ is_ok Gk.ia G2.ca Gk.i_k /\
+                              is_ok Ok.is Ok.cs Ok.ik])).
+byequiv (: ={arg, glob Dkx} /\ arg{1} = (x, y) ==> _) => //.
+conseq (Ok_Okx &m x y Dkx x_EU y_EU Dkx_ll Dkx_initP); smt().
+byequiv (: ={glob A, x, y} /\ fst arg{1} = x /\ snd arg{1} = y ==> _) => //.
+proc; inline *; wp.
+call (: ={OAEU.m, G2.ca, G.bad} /\ ={m}(OEU, OBEU) /\
+        ={cddh, i_k, k, ia, ib}(Gk, Gk) /\ ={x}(GkxD, Gkx) /\
+        Ok.cs{1} = G2.cb{2} /\ Ok.ik{1} = Gk.j_k{2} /\
+        Ok.is{1} = Gk.ib{2} /\ Ok.x{1} = Gkx.y{2} /\
+        (G.bad = Ok.bad /\ Ok.n = nb){1});
+  1..4: (by proc; inline *; sp; if; try if; auto); 2: by auto.
+- proc; inline Gkxy(OAEU, OBEU).ddh Count(GkxD(OAEU, O_i_O(Okx(OEU)))).ddh.
+  inline GkxD(OAEU, O_i_O(Okx(OEU))).ddh O_i_O(Ok(OEU)).get_cs.
+  sp; if; 1, 3: by auto.
+  seq 4 3 : (={OAEU.m, G2.ca, G.bad, t} /\ ={m}(OEU, OBEU) /\
+             ={cddh, i_k, k, ia, ib}(Gk, Gk) /\ ={x}(GkxD, Gkx) /\
+             Ok.cs{1} = G2.cb{2} /\ Ok.ik{1} = Gk.j_k{2} /\
+             Ok.is{1} = Gk.ib{2} /\ Ok.x{1} = Gkx.y{2} /\
+             (G.bad = Ok.bad /\ Ok.n = nb){1} /\
+             i1{1} = i0{2} /\ j1{1} = j0{2} /\ r1{1} = r0{2} /\
+             cb{1} = G2.cb{2} /\ 0 <= j1{1} < nb); 2: by inline *; auto => />.
+  swap 1 1; wp; call (: ={OAEU.m}); auto.
+  by inline *; sp; rcondt{1} 1; auto; smt(expM mulC).
+qed.
+
+local lemma Gkxy_S &m x y :
+  x \in EU =>
+  y \in EU =>
+  Pr[Game_xy(Gkxy(OAEU, OBEU), A).main(x, y) @ &m :
+     G.bad /\ is_ok Gk.ia G2.ca Gk.i_k /\ is_ok Gk.ib G2.cb Gk.j_k] <=
+  Pr[GameS(A).main(exp g x, exp g y) @ &m : S.m_crit = exp g (x * y)].
+proof.
+move => x_EU y_EU; byequiv => //; proc; inline *; symmetry.
+call (: ! nstop Gk.ia Gk.ib G2.ca G2.cb \/
+        ! (G.bad => nth false Gk.ia Gk.i_k /\ nth false Gk.ib Gk.j_k) \/
+        Gk.k <= Gk.cddh,
+
+        ={OAEU.m, OBEU.m, G2.ca, G2.cb} /\ ={cddh, k, ia, ib}(S, Gk) /\
+        (S.gx = exp g x /\ S.gy = exp g y){1} /\
+        (Gkx.x = x /\ Gkx.y = y){2} /\
+        (G.bad{2} => S.m_crit{1} = exp g (x * y)) /\
+        (G.bad <=> Gk.k <= Gk.cddh){2} /\
+        (forall i, i \in OAEU.m => oget (OAEU.m.[i]) \in EU){2} /\
+        (forall j, j \in OBEU.m => oget (OBEU.m.[j]) \in EU){2},
+
+        ! ( nstop Gk.ia Gk.ib G2.ca G2.cb){2} \/
+        ! (G.bad => nth false Gk.ia Gk.i_k /\ nth false Gk.ib Gk.j_k){2} \/
+        (S.k <= S.cddh /\ S.m_crit = exp g (x * y)){1} \/
+        (Gk.k <= Gk.cddh /\ ! G.bad){2});
+  2, 5: by proc; inline *; sp; if; auto;
+           smt(expM exp_inv get_setE get_set_sameE memE mulA supp_duniform).
+- by exact A_ll.
+- by move => *; proc; inline *; sp; if; auto; smt(dEU_ll).
+- by move => *; proc; inline *; sp; if; auto; smt(dEU_ll).
+- by move => *; proc; inline *; sp; if; auto; smt(dEU_ll).
+- by move => *; proc; inline *; sp; if; auto; smt(dEU_ll).
+- by proc; inline *; sp; if; [ | if; auto | ]; auto;
+     smt(expM get_setE get_set_sameE supp_duniform memE).
+- by move => *; proc; inline *; sp; if; auto; if; auto; smt(dEU_ll).
+- by move => *; proc; inline *; sp; if; auto; if; auto; smt(dEU_ll).
+- by proc; inline *; sp; if; [ | if; auto | ]; auto;
+     smt(expM get_setE get_set_sameE supp_duniform memE).
+- by move => *; proc; inline *; sp; if; auto; if; auto; smt(dEU_ll).
+- by move => *; proc; inline *; sp; if; auto; if; auto; smt(dEU_ll).
+- proc; inline S.ddh Gkxy(RAEU.RO, RBEU.RO).ddh.
+  sp 8 9; if; [smt() | | auto; smt()].
+  seq 2 2 : (={m0, i0, j0, a, b, r0} /\ a{2} \in EU /\ b{2} \in EU /\
+             ( nstop Gk.ia Gk.ib G2.ca G2.cb){2} /\
+             ={OAEU.m, OBEU.m, G2.ca, G2.cb} /\ ={cddh, k, ia, ib}(S, Gk) /\
+             (S.gx = exp g x /\ S.gy = exp g y){1} /\
+             (Gkx.x = x /\ Gkx.y = y){2} /\
+             (! G.bad /\ Gk.cddh <= Gk.k){2} /\
+             (forall i, i \in OAEU.m => oget (OAEU.m.[i]) \in EU){2} /\
+             (forall j, j \in OBEU.m => oget (OBEU.m.[j]) \in EU){2});
+    1: by inline *; auto; smt(get_setE get_set_sameE memE supp_duniform).
+  auto => /> &2; move: (i0{2}) (j0{2}) (G2.ca{2}) (G2.cb{2}) => i j ca cb *.
+  (case: (i \in ca) => [i_ca | iNca]); (case: (j \in cb) => [j_cb | jNcb] /=);
+    1..3: smt(expM mulA mulC).
+  rewrite -implybE -!expM => [cddh_k [-> ->] /=].
+  have -> : x * a{2} * (y * b{2}) * (inv a{2} * inv b{2}) =
+            (a{2} * inv a{2}) * (b{2} * inv b{2} * (x * y)) by smt(mulA mulC).
+  by rewrite !exp_inv.
+- move => &2 *.
+  conseq (: _ ==> true) (: _ ==> _) => //; 2: by islossless.
+  proc; inline S.ddh; sp; elim * => cddh Ccddh.
+  if; 2: by auto; smt().
+  by inline *; auto; smt(get_setE get_set_sameE memE supp_duniform).
+- move => &1.
+  conseq (: _ ==> true) (: _ ==> _) => //; 2: by islossless.
+  proc; inline Gkxy(RAEU.RO, RBEU.RO).ddh; sp; elim * => cddh Ccddh.
+  if; 2: by auto; smt().
+  by inline *; auto; smt(get_setE get_set_sameE memE supp_duniform).
+- auto => />; smt(mem_empty supp_dinter).
+qed.
+
+local lemma A_B &m :
+  Pr[Game(Gk(OAEU, OBEU), A).main() @ &m :
+     G.bad /\ is_ok Gk.ia G2.ca Gk.i_k /\ is_ok Gk.ib G2.cb Gk.j_k] <=
+  Pr[NCDH.Game(B(A)).main() @ &m : res].
+proof.
+pose p := Pr[Game(Gk(OAEU,OBEU), A).main() @ &m :
+             G.bad /\ is_ok Gk.ia G2.ca Gk.i_k /\ is_ok Gk.ib G2.cb Gk.j_k].
+byphoare (: (glob A, Gk.i_k, Gk.j_k) = (glob A, Gk.i_k, Gk.j_k){m} ==> _) => //.
+proc; inline B(A).solve; wp.
+seq 4 : true 1%r p 0%r _
+        (x \in EU /\ y \in EU /\ gx = exp g x /\ gy = exp g y /\
+        (glob A, Gk.i_k, Gk.j_k) = (glob A, Gk.i_k, Gk.j_k){m}) => //.
+- by auto => />; smt(memE supp_duniform).
+- by islossless; apply duniform_ll; smt(e_EU).
+exlim x, y => x' y'.
+call (: (x' \in EU) /\ (y' \in EU) /\ gx = exp g x' /\ gy = exp g y' /\
+        (glob A, Gk.i_k, Gk.j_k) = (glob A, Gk.i_k, Gk.j_k){m} ==>
+        S.m_crit = exp g (x' * y')); 2: by auto.
+bypr => &m' /> 2? -> -> *.
+have -> : p = Pr[Game(Gk(OAEU,OBEU), A).main() @ &m' :
+                 G.bad /\ is_ok Gk.ia G2.ca Gk.i_k /\ is_ok Gk.ib G2.cb Gk.j_k].
+  by rewrite /p; byequiv => //; sim => /> /#.
+by apply (ler_trans _ _ _ _ (Gkxy_S &m' x' y' _ _)) => //; smt(Gk_Gkx Gkx_Gkxy).
+qed.
+
+lemma G1G2_NCDH &m :
+  `| Pr[ Game(G1, A).main() @ &m : res] - Pr[ Game(G2, A).main() @ &m : res] | <=
+  q_ddh%r / ((1%r - pa) ^ q_oa * (1%r - pb) ^ q_ob * pa * pb) *
+  Pr[NCDH.Game(B(A)).main() @ &m : res] + DELTA.
+proof.
+apply (ler_trans _ _ _ (G1G2_Gbad &m) _).
+suff: Pr[Game(G', A).main() @ &m : G.bad] <=
+      q_ddh%r / ((1%r - pa) ^ q_oa * (1%r - pb) ^ q_ob * pa * pb) *
+      Pr[NCDH.Game(B(A)).main() @ &m : res] by smt(G_G').
+have H1 := guess_bound &m; have H2 := A_B &m.
+have {H1 H2} H := ler_trans _ _ _ H1 H2.
+rewrite -ler_pdivr_mull; 2: by rewrite invf_div; smt().
+by smt(divr_gt0 expr0 expr_gt0 mulr_gt0 pa_bound pb_bound q_ddh_ge1).
+qed.
+
+end section.
+
+end Inner.
+
+(* The optimal bound is obtained by setting pa = 1/(q_oa + 1) and likewise for pb *)
+
+lemma pa_bound :
+  0%r < (1%r/(q_oa + 1)%r) &&
+  if q_oa = 0 then (1%r/(q_oa + 1)%r) <= 1%r else (1%r/(q_oa + 1)%r) < 1%r.
+proof. smt. qed.
+
+lemma pb_bound :
+  0%r < (1%r/(q_ob + 1)%r) &&
+  if q_ob = 0 then (1%r/(q_ob + 1)%r) <= 1%r else (1%r/(q_ob + 1)%r) < 1%r.
+proof. smt. qed.
+
+clone import Inner as I with
+  op pa <- (1%r/(q_oa + 1)%r),
+  op pb <- (1%r/(q_ob + 1)%r),
+  axiom pa_bound <- pa_bound, (* does anything break/change if we remove this? *)
+  axiom pb_bound <- pb_bound.
+
+(* Need to find a better name *)
+lemma foo_monotone (n m : int) :
+  0 <= n => n <= m => (n%r/(n+1)%r)^(n+1) <= (m%r/(m+1)%r)^(m+1).
+proof.
+suff nP : forall n, 0 <= n =>
+                    (n%r / (n + 1)%r) ^ (n + 1) <=
+                    ((n + 1)%r / (n + 1 + 1)%r) ^ (n + 1 + 1).
+- move => n_ge0; rewrite StdOrder.IntOrder.ler_eqVlt; move => [<- /#|mP].
+  have {mP} [q] : (exists q, m - n = q /\ 0 < q) by smt ().
+  have [p] : exists p, p = q - 1 by smt().
+  rewrite eq_sym subr_eq => ->; rewrite subr_eq addrC.
+  move => {q} [-> pP]; have {pP} pP : 0 <= p by smt().
+  elim: p pP; 1: smt().
+  move => i i_ge0 iP; apply (ler_trans _ _ _ iP).
+  apply (ler_trans (((n+i+1)%r/((n+i+1)+1)%r)^((n+i+1)+1))); 1: smt().
+  have {i_ge0 n_ge0} n_ge0 : 0<= n + i + 1 by smt().
+  by apply (ler_trans _ _ _ (nP _ n_ge0)); smt().
+- move => {m n} n; rewrite StdOrder.IntOrder.ler_eqVlt; move => [<-|n_gt0];
+    1: by rewrite add0r mul0r exprSr // !expr1; smt(mulr_ge0).
+  have -> : ((n + 1)%r / (n + 1 + 1)%r) ^ (n + 1 + 1) =
+            (n%r / (n + 1)%r) ^ (n + 1) * ((n + 1)%r / (n + 2)%r) *
+            ((n + 1)%r ^2 / (n%r * (n + 2)%r)) ^ (n + 1).
+  + rewrite mulrAC -exprMn; 1: smt().
+    suff -> : n%r / (n + 1)%r * ((n + 1)%r ^ 2 / (n%r * (n + 2)%r)) =
+              (n + 1)%r / (n + 2)%r by smt(exprSr).
+    by rewrite expr2; algebra; smt(expr2).
+  have {1}-> : (n%r/(n+1)%r)^(n+1) = (n%r/(n+1)%r)^(n+1)*1%r by smt().
+  rewrite -subr_ge0 -!mulrA -mulrBr mulr_ge0; 1: smt(expr_gt0).
+  rewrite subr_ge0 -ler_pdivr_mull; 1: smt().
+  rewrite -ler_pdivr_mull; 1: smt().
+  apply (ler_trans (1%r + 1%r / (n + 1)%r));
+    1: by rewrite -subr_ge0 le0r; left; algebra; smt().
+  have -> : (n + 1)%r ^ 2 / (n%r * (n + 2)%r) = 1%r + 1%r / (n%r * (n + 2)%r)
+    by algebra; smt(expr2).
+  apply (ler_trans (1%r + (n + 1)%r / (n%r * (n + 2)%r))).
+  + suff : 1%r / (n + 1)%r <= (n + 1)%r / (n%r * (n + 2)%r) by smt().
+    rewrite -ler_pdivl_mulr; 1: smt().
+    apply (ler_trans ((n + 1)%r ^ 2 / (n%r * (n + 2)%r))).
+    * move: (subr_sqr_1 (n + 1)%r); rewrite subr_eq => ->.
+      rewrite ler_pdivl_mulr ?mul1r; 1: smt().
+      suff: n%r * (n + 2)%r <= ((n + 1)%r - 1%r) * ((n + 1)%r + 1%r); 1: smt().
+      by rewrite -fromintD -fromintB; smt().
+    * by rewrite -subr_ge0 le0r; left; algebra; smt(expr2).
+  + rewrite Binomial.BCR.binomial; 1: smt().
+    rewrite 2?rangeSr; 1, 2: smt().
+    rewrite !StdBigop.Bigreal.BRA.big_rcons /predT /=.
+    rewrite -addrA Binomial.binn; 1: smt().
+    apply ler_paddl.
+    * apply StdBigop.Bigreal.sumr_ge0_seq.
+      move => a aP _; rewrite mulr_ge0; 1: smt(Binomial.ge0_bin).
+      by rewrite expr1z mul1r; smt(expr_gt0).
+    * have -> : n + 1 - n = 1 by algebra.
+      rewrite !expr1z expr0 expr1 !mul1r.
+      suff -> : (Binomial.bin (n + 1) n)%Binomial = n + 1 by smt().
+      have {n_gt0} n_ge0 : 0 <= n by smt().
+      elim: n n_ge0; 1: smt(Binomial.bin0).
+      move => n n_ge0 nP; rewrite Binomial.binSn; 1, 2: smt().
+      by rewrite nP Binomial.binn; smt().
+qed.
+
+section.
+
+declare module A : Adversary {G1, G2, G, S, Count,
+                              OAEU, OBEU, OEU, O0EU, O1EU, O1G}.
+
+axiom A_ll : forall (O <: CDH_RSR_Oracles{A}),
+  islossless O.oA =>
+  islossless O.oB =>
+  islossless O.oa =>
+  islossless O.ob =>
+  islossless O.ddh =>
+  islossless A(O).guess.
+
+axiom A_bound : forall (O <: CDH_RSR_Oracles{A}),
+  hoare [A(Count(O)).guess :
+         Count.ca = 0 /\ Count.cb = 0 /\ Count.cddh = 0 ==>
+         Count.ca <= q_oa /\ Count.cb <= q_ob /\ Count.cddh <= q_ddh].
+
+lemma G1G2_NCDH &m :
+  `| Pr[Game(G1,A).main() @ &m : res] - Pr[ Game(G2,A).main() @ &m : res] | <=
+  q_ddh%r * (max 1 (4*q_oa))%r * (max 1 (4 * q_ob))%r *
+  Pr[NCDH.Game(B(A)).main() @ &m : res] + DELTA.
+proof.
+have H := I.G1G2_NCDH (<:A) A_ll A_bound &m.
+apply (ler_trans _ _ _ H) => {H}.
+suff Hmax : forall (n : int),
+              0 <= n =>
+              1%r/((1%r-1%r/(n+1)%r)^n*(1%r/(n+1)%r)) <= (max 1 (4*n))%r.
+- rewrite ler_add2r ler_wpmul2r; 1: smt.
+  rewrite -!mulrA ler_wpmul2l; 1: smt(q_ddh_ge1).
+  apply (ler_trans ((1%r/((1%r-1%r/(q_oa+1)%r)^q_oa*(1%r/(q_oa+1)%r))) *
+                    (1%r/((1%r-1%r/(q_ob+1)%r)^q_ob*(1%r/(q_ob+1)%r)))));
+    1: smt.
+  apply ler_pmul; smt(q_oa_ge0 q_ob_ge0 divr_ge0 expr_ge0 invr_ge0 mulr_ge0).
+- move => n n_ge0; case (n = 0) => [-> /=|H]; 1: smt(expr0).
+  have {H n_ge0} n_gt0 : 1 <= n by smt().
+  apply (ler_trans (4 * n)%r); 2: smt().
+  rewrite ler_pdivr_mulr; 1: smt (divr_gt0 expr_gt0 mulr_gt0).
+  rewrite mulrC -ler_pdivr_mulr; 1: smt().
+  have -> : 1%r / (4 * n)%r = (1%r /(1 + 1)%r)^(1 + 1) * (1%r / n%r)
+    by rewrite !div1r expr2 -!invfM fromintD fromintM mulrDl mul1r -addrA.
+  suff -> : (1%r - 1%r / (n + 1)%r) ^ n * (1%r / (n + 1)%r) =
+            (n%r / (n + 1)%r)^(n + 1) * (1%r / n%r)
+    by rewrite ler_wpmul2r; [smt(divr_ge0)|by apply foo_monotone].
+  apply (can2_eq (fun x, x * (1%r / (n + 1)%r)) (fun x, x * (n + 1)%r)) => /=;
+    1, 2: by move => x; smt(divrr).
+  rewrite -mulrA exprSr; 1: smt().
+  rewrite- mulrA -{2}invf_div divrr ?mulr1; 1: smt().
+  suff: 1%r - inv (n + 1)%r = n%r / (n + 1)%r; smt.
+qed.
+
+end section.
