theories/crypto/NominalGroup.ec
@@ -1,0 +1,62 @@
+(* -------------------------------------------------------------------- *)
+require import AllCore Distr List IntMin IntDiv.
+require import FinType FSet.
+require (*--*) Ring Number StdOrder ZModP.
+
+import Ring.IntID StdOrder.IntOrder.
+
+(* -------------------------------------------------------------------- *)
+
+op injective_on (A : 'a fset) (f : 'a -> 'b) : bool =
+  forall (x y : 'a), x \in A => y \in A => f x = f y => x = y.
+
+abstract theory NominalGroup.
+
+type G.
+type Z.
+
+clone include FinType
+  with type t <- G
+  rename "card" as "order"
+  rename "enum" as "elems".
+
+op g     : G.
+op ( ^ ) : G -> Z -> G.
+
+op ( * ) : Z -> Z -> Z.
+op inv   : Z -> Z.
+
+op f : Z.
+op exp (a, x) = a ^ (x * inv f).
+
+op EU : Z fset.
+op dZ : Z distr.
+
+axiom dZ_ll : is_lossless dZ.
+hint exact random : dZ_ll.
+
+axiom mulA       : associative ( * ).
+axiom mulC       : commutative ( * ).
+
+axiom powM       : forall a x y, a ^ (x * y) = (a ^ x) ^ y.
+axiom pow_inv    : forall x, x \in EU => g ^ (x * inv x) = g.
+axiom pow_inv_f  : forall a, a ^ (f * inv f) = a.
+
+axiom exp_inj    : injective_on EU (exp g).
+axiom exp_inj'   : forall x, injective_on EU (fun z => exp g (x * z)).
+
+axiom img_exp    : forall x, x \in EU =>
+                             image (fun z => exp g (x * z)) EU =
+                             image (exp g) EU.
+
+lemma expM a x y : exp a (x * y) = (exp a x) ^ y.
+proof. by rewrite /exp -!powM -!mulA (mulC y). qed.
+
+lemma exp_inv x y : x \in EU => exp g (x * inv x * y) = exp g y.
+proof.
+move => x_EU; rewrite /exp.
+have -> : x * inv x * y * inv f = (x * inv x) * (y * inv f) by smt(mulA mulC).
+by rewrite powM pow_inv.
+qed.
+
+end NominalGroup.
