theories/crypto/SplitRO2.ec
@@ -1,0 +1,144 @@
+require import AllCore PROM SmtMap Distr DProd.
+
+abstract theory Split.
+
+  type in_t,out_t,d_in_t,d_out_t.
+
+  op dout : in_t -> out_t distr.
+
+  clone import FullRO as IdealAll with
+    type in_t    <- in_t,
+    type out_t   <- out_t,
+    type d_in_t  <- d_in_t,
+    type d_out_t <- d_out_t,
+    op   dout    <- dout.
+
+abstract theory SplitDomT.
+
+module type ROt = {
+  include RO [-init]
+  proc init (_ : in_t -> bool) : unit
+}.
+
+abstract theory MkROt.
+module RO : ROt = {
+  var m : (in_t, out_t) fmap
+
+  proc init (t : in_t -> bool) = {
+    m <- empty;
+  }
+
+  proc get (x : in_t) = {
+    var r;
+
+    r <$ dout x;
+    if (x \notin m) {
+      m.[x] <- r;
+    }
+    return (oget m.[x]);
+  }
+
+  proc set (x : in_t, y : out_t) = {
+    m.[x] <- y;
+  }
+
+  proc rem (x : in_t) = {
+    m <- rem m x;
+  }
+
+  proc sample (x : in_t) = {
+    get(x);
+  }
+
+  proc restrK () = {
+    return m;
+  }
+}.
+end MkROt.
+
+clone include MkROt.
+
+module type RO_DistinguisherT (G : ROt) = {
+  proc get_test () : in_t -> bool {}
+  proc distinguish (_ : d_in_t): d_out_t
+}.
+
+module MainDT (D : RO_DistinguisherT) (RO : ROt) = {
+  proc distinguish (x) = {
+    var t, r;
+
+    t <@ D(RO).get_test();
+    RO.init(t);
+    r <@ D(RO).distinguish(x);
+    return r;
+  }
+}.
+
+
+module RO_DOMt (ROT : RO) (ROF: RO) : ROt = {
+  var test : in_t -> bool
+
+  proc init (test': in_t -> bool) = { test <- test'; ROT.init(); ROF.init(); }
+
+  proc get (x : in_t) = {
+    var r;
+    if (test x) r <@ ROT.get(x);
+    else r <@ ROF.get(x);
+    return r;
+  }
+
+  proc set (x : in_t, y : out_t) = {
+    if (test x) ROT.set(x, y);
+    else ROF.set(x, y);
+  }
+
+  proc rem (x : in_t) = {
+    if (test x) ROT.rem(x);
+    else ROF.rem(x);
+  }
+
+  proc sample (x : in_t) = {
+    if (test x) ROT.sample(x);
+    else ROF.sample(x);
+  }
+}.
+
+clone MkRO as ROT.
+clone MkRO as ROF.
+
+section PROOFS.
+
+declare module D: RO_DistinguisherT {RO, RO_DOMt, ROT.RO, ROF.RO}.
+
+equiv RO_split :
+  MainDT(D, RO).distinguish ~ MainDT(D, RO_DOMt(ROT.RO, ROF.RO)).distinguish :
+  ={arg, glob D} ==>
+  ={res, glob D} /\ RO.m{1} = union_map ROT.RO.m{2} ROF.RO.m{2} /\
+  (forall x, x \in ROT.RO.m{2} =>   RO_DOMt.test{2} x) /\
+  (forall x, x \in ROF.RO.m{2} => ! RO_DOMt.test{2} x).
+proof.
+  proc.
+  call (_ : RO.m{1} = union_map ROT.RO.m{2} ROF.RO.m{2} /\
+            (forall x, x \in ROT.RO.m{2} =>   RO_DOMt.test{2} x) /\
+            (forall x, x \in ROF.RO.m{2} => ! RO_DOMt.test{2} x)).
+  - proc; inline *.
+    if {2}; auto=> />; 2: smt(get_setE mergeE set_union_map_r).
+    by smt(get_setE mem_union_map mergeE set_union_map_l).
+  - proc; inline *.
+    if {2}; auto=> />; 2: smt(get_setE mergeE set_union_map_r).
+    by smt(get_setE mem_union_map mergeE set_union_map_l).
+  - by proc; inline *; auto=> />; smt(mem_rem rem_id rem_merge).
+  - proc; inline *.
+    if {2}; auto=> />; 2: smt(get_setE mergeE set_union_map_r).
+    by smt(get_setE mem_union_map mergeE set_union_map_l).
+  - proc; inline *; auto => />.
+    by rewrite {1}/union_map merge_empty //; smt(mem_empty).
+  - inline *; auto; call(: true) => />; 1: by move=> /> /#.
+    by skip => /> r; rewrite {1}/union_map merge_empty //; smt(mem_empty).
+qed.
+
+end section PROOFS.
+
+end SplitDomT.
+
+end Split.
